Added ext fn to implementation for testing

noc.ml
@@ -95,7 +95,8 @@ module Nat =
       (fun _ -> p)
       (fun k' ->
       (fun fO fS n -> if n=0 then fO () else fS (n-1))
-        (fun _ -> log2_iter k' (Stdlib.Int.succ p) (Stdlib.Int.succ q) q)
+        (fun _ ->
+        log2_iter k' (Stdlib.Int.succ p) (Stdlib.Int.succ q) q)
         (fun r' -> log2_iter k' p (Stdlib.Int.succ q) r')
         r0)
       k
@@ -174,9 +175,10 @@ let rec fold_right f a0 = function
 let rec combine l l' =
   match l with
   | [] -> []
-  | x :: tl -> (match l' with
-                | [] -> []
-                | y :: tl' -> (x, y) :: (combine tl tl'))
+  | x :: tl ->
+    (match l' with
+     | [] -> []
+     | y :: tl' -> (x, y) :: (combine tl tl'))
 
 (** val skipn : int -> 'a1 list -> 'a1 list **)
 
@@ -315,7 +317,8 @@ let rec vect_nth n0 v idx =
 let rec vect_map n0 f v =
   (fun fO fS n -> if n=0 then fO () else fS (n-1))
     (fun _ -> Obj.magic __ v)
-    (fun n1 -> vect_cons n1 (f (vect_hd n1 v)) (vect_map n1 f (vect_tl n1 v)))
+    (fun n1 ->
+    vect_cons n1 (f (vect_hd n1 v)) (vect_map n1 f (vect_tl n1 v)))
     n0
 
 (** val vect_find_index : int -> ('a1 -> bool) -> 'a1 vect -> index option **)
@@ -341,14 +344,16 @@ let vect_index sz0 eQ k v =
 let eqDec_vect_nil _ =
   { eq_dec = (fun _ _ -> true) }
 
-(** val eqDec_vect_cons : 'a1 eqDec -> 'a2 eqDec -> ('a1, 'a2) vect_cons_t eqDec **)
+(** val eqDec_vect_cons :
+    'a1 eqDec -> 'a2 eqDec -> ('a1, 'a2) vect_cons_t eqDec **)
 
 let eqDec_vect_cons h h0 =
   { eq_dec = (fun t1 t2 ->
     let vhd0 = t1.vhd in
     let vtl0 = t1.vtl in
     let vhd1 = t2.vhd in
-    let vtl1 = t2.vtl in if h.eq_dec vhd0 vhd1 then h0.eq_dec vtl0 vtl1 else false) }
+    let vtl1 = t2.vtl in
+    if h.eq_dec vhd0 vhd1 then h0.eq_dec vtl0 vtl1 else false) }
 
 (** val eqDec_vect : int -> 'a1 eqDec -> 'a1 vect eqDec **)
 
@@ -424,7 +429,8 @@ type ('s, 'f) result =
 | Success of 's
 | Failure of 'f
 
-(** val result_map_failure : ('a2 -> 'a3) -> ('a1, 'a2) result -> ('a1, 'a3) result **)
+(** val result_map_failure :
+    ('a2 -> 'a3) -> ('a1, 'a2) result -> ('a1, 'a3) result **)
 
 let result_map_failure fn = function
 | Success s -> Success s
@@ -461,7 +467,8 @@ type 'k member =
 | MemberTl of 'k * 'k * 'k list * 'k member
 
 (** val assoc :
-    'a1 eqDec -> 'a1 -> ('a1 * 'a2) list -> ('a2, ('a1 * 'a2) member) sigT option **)
+    'a1 eqDec -> 'a1 -> ('a1 * 'a2) list -> ('a2, ('a1 * 'a2) member) sigT
+    option **)
 
 let rec assoc h k1 = function
 | [] -> None
@@ -501,10 +508,12 @@ let rec list_nth l idx =
        (fun a -> list_nth l0 a)
        (Obj.magic idx))
 
-type 'a struct_sig' = { struct_name : char list; struct_fields : (char list * 'a) list }
+type 'a struct_sig' = { struct_name : char list;
+                        struct_fields : (char list * 'a) list }
 
-type enum_sig = { enum_name : char list; enum_size : int; enum_bitsize : int;
-                  enum_members : char list vect; enum_bitpatterns : bool vect vect }
+type enum_sig = { enum_name : char list; enum_size : int; enum_bitsize : 
+                  int; enum_members : char list vect;
+                  enum_bitpatterns : bool vect vect }
 
 type 'a array_sig' = { array_type : 'a; array_len : int }
 
@@ -528,7 +537,8 @@ let kind_of_type = function
 | Struct_t sig0 -> Kind_struct (Some sig0)
 | Array_t sig0 -> Kind_array (Some sig0)
 
-(** val struct_fields_sz' : (type0 -> int) -> (char list * type0) list -> int **)
+(** val struct_fields_sz' :
+    (type0 -> int) -> (char list * type0) list -> int **)
 
 let struct_fields_sz' type_sz0 fields =
   list_sum (map (fun nm_tau -> type_sz0 (snd nm_tau)) fields)
@@ -582,7 +592,8 @@ let element_sz sig0 =
 (** val element_offset_right : type0 array_sig' -> array_index -> int **)
 
 let element_offset_right sig0 idx =
-  Bits.rmul (sub sig0.array_len (Stdlib.Int.succ (index_to_nat sig0.array_len idx)))
+  Bits.rmul
+    (sub sig0.array_len (Stdlib.Int.succ (index_to_nat sig0.array_len idx)))
     (element_sz sig0)
 
 type port =
@@ -593,24 +604,31 @@ type type_denote = __
 
 type 'argKind _Sig = { argSigs : 'argKind vect; retSig : 'argKind }
 
+type ('argKind, 'type_of_argKind) _Sig_denote = __
+
+type sig_denote = (type0, type_denote) _Sig_denote
+
 (** val cSig_of_Sig : int -> type0 _Sig -> int _Sig **)
 
 let cSig_of_Sig n0 sig0 =
-  { argSigs = (vect_map n0 type_sz sig0.argSigs); retSig = (type_sz sig0.retSig) }
+  { argSigs = (vect_map n0 type_sz sig0.argSigs); retSig =
+    (type_sz sig0.retSig) }
 
 (** val sig_of_CSig : int -> int _Sig -> type0 _Sig **)
 
 let sig_of_CSig n0 sig0 =
-  { argSigs = (vect_map n0 (fun x -> Bits_t x) sig0.argSigs); retSig = (Bits_t
-    sig0.retSig) }
+  { argSigs = (vect_map n0 (fun x -> Bits_t x) sig0.argSigs); retSig =
+    (Bits_t sig0.retSig) }
 
 type externalSignature = type0 _Sig
 
 type 'var_t tsig = ('var_t * type0) list
 
 type ('var_t, 'fn_name_t, 'action) internalFunction = { int_name : 'fn_name_t;
-                                                        int_argspec : 'var_t tsig;
-                                                        int_retSig : type0;
+                                                        int_argspec : 
+                                                        'var_t tsig;
+                                                        int_retSig : 
+                                                        type0;
                                                         int_body : 'action }
 
 (** val map_intf_body :
@@ -618,8 +636,8 @@ type ('var_t, 'fn_name_t, 'action) internalFunction = { int_name : 'fn_name_t;
     internalFunction **)
 
 let map_intf_body f fn =
-  { int_name = fn.int_name; int_argspec = fn.int_argspec; int_retSig = fn.int_retSig;
-    int_body = (f fn.int_body) }
+  { int_name = fn.int_name; int_argspec = fn.int_argspec; int_retSig =
+    fn.int_retSig; int_body = (f fn.int_body) }
 
 type 'var_t arg_sig = { arg_name : 'var_t; arg_type : type0 }
 
@@ -641,13 +659,13 @@ let eqDec_type =
        | Enum_t sig0 ->
          (match t2 with
           | Enum_t sig1 ->
-            let { enum_name = enum_name0; enum_size = enum_size0; enum_bitsize =
-              enum_bitsize0; enum_members = enum_members0; enum_bitpatterns =
-              enum_bitpatterns0 } = sig0
+            let { enum_name = enum_name0; enum_size = enum_size0;
+              enum_bitsize = enum_bitsize0; enum_members = enum_members0;
+              enum_bitpatterns = enum_bitpatterns0 } = sig0
             in
-            let { enum_name = enum_name1; enum_size = enum_size1; enum_bitsize =
-              enum_bitsize1; enum_members = enum_members1; enum_bitpatterns =
-              enum_bitpatterns1 } = sig1
+            let { enum_name = enum_name1; enum_size = enum_size1;
+              enum_bitsize = enum_bitsize1; enum_members = enum_members1;
+              enum_bitpatterns = enum_bitpatterns1 } = sig1
             in
             let s = eqDec_string.eq_dec enum_name0 enum_name1 in
             if s
@@ -656,8 +674,8 @@ let eqDec_type =
                  then let s1 = eqDec_nat.eq_dec enum_bitsize0 enum_bitsize1 in
                       if s1
                       then let s2 =
-                             (eqDec_vect enum_size1 eqDec_string).eq_dec enum_members0
-                               enum_members1
+                             (eqDec_vect enum_size1 eqDec_string).eq_dec
+                               enum_members0 enum_members1
                            in
                            if s2
                            then (eqDec_vect enum_size1
@@ -671,9 +689,11 @@ let eqDec_type =
        | Struct_t sig0 ->
          (match t2 with
           | Struct_t sig1 ->
-            let { struct_name = struct_name0; struct_fields = struct_fields0 } = sig0
+            let { struct_name = struct_name0; struct_fields =
+              struct_fields0 } = sig0
             in
-            let { struct_name = struct_name1; struct_fields = struct_fields1 } = sig1
+            let { struct_name = struct_name1; struct_fields =
+              struct_fields1 } = sig1
             in
             let s = eqDec_string.eq_dec struct_name0 struct_name1 in
             if s
@@ -688,7 +708,9 @@ let eqDec_type =
                       | p :: l1 ->
                         if let (a, b) = y in
                            let (s0, t) = p in
-                           if eqDec_string.eq_dec a s0 then iHtau b t else false
+                           if eqDec_string.eq_dec a s0
+                           then iHtau b t
+                           else false
                         then f l0 l1
                         else false)
                  in f struct_fields0 struct_fields1
@@ -752,7 +774,8 @@ let assert_kind kind arg tau =
      | _ -> Failure (arg, (KindMismatch ((kind_of_type tau), kind))))
 
 type ('pos_t, 'var_t, 'fn_name_t) error = { epos : 'pos_t;
-                                            emsg : ('var_t, 'fn_name_t) error_message }
+                                            emsg : ('var_t, 'fn_name_t)
+                                                   error_message }
 
 type bits_comparison =
 | CLt
@@ -891,22 +914,26 @@ module PrimTyped =
   (** val coq_GetElementBits : type0 array_sig' -> array_index -> fbits1 **)
 
   let coq_GetElementBits sig0 idx =
-    Slice ((array_sz sig0), (element_offset_right sig0 idx), (element_sz sig0))
+    Slice ((array_sz sig0), (element_offset_right sig0 idx),
+      (element_sz sig0))
 
   (** val coq_SubstElementBits : type0 array_sig' -> array_index -> fbits2 **)
 
   let coq_SubstElementBits sig0 idx =
-    SliceSubst ((array_sz sig0), (element_offset_right sig0 idx), (element_sz sig0))
+    SliceSubst ((array_sz sig0), (element_offset_right sig0 idx),
+      (element_sz sig0))
 
   (** val coq_GetFieldBits : type0 struct_sig' -> struct_index -> fbits1 **)
 
   let coq_GetFieldBits sig0 idx =
-    Slice ((struct_sz sig0), (field_offset_right sig0 idx), (field_sz sig0 idx))
+    Slice ((struct_sz sig0), (field_offset_right sig0 idx),
+      (field_sz sig0 idx))
 
   (** val coq_SubstFieldBits : type0 struct_sig' -> struct_index -> fbits2 **)
 
   let coq_SubstFieldBits sig0 idx =
-    SliceSubst ((struct_sz sig0), (field_offset_right sig0 idx), (field_sz sig0 idx))
+    SliceSubst ((struct_sz sig0), (field_offset_right sig0 idx),
+      (field_sz sig0 idx))
  end
 
 module PrimTypeInference =
@@ -915,16 +942,18 @@ module PrimTypeInference =
       type0 struct_sig' -> char list -> (index, fn_tc_error) result **)
 
   let find_field sig0 f =
-    opt_result (list_assoc eqDec_string f sig0.struct_fields) (Arg1, (UnboundField (f,
-      sig0)))
+    opt_result (list_assoc eqDec_string f sig0.struct_fields) (Arg1,
+      (UnboundField (f, sig0)))
 
   (** val check_index :
       type0 array_sig' -> int -> (array_index, fn_tc_error) result **)
 
   let check_index sig0 pos =
-    opt_result (index_of_nat sig0.array_len pos) (Arg1, (OutOfBounds (pos, sig0)))
+    opt_result (index_of_nat sig0.array_len pos) (Arg1, (OutOfBounds (pos,
+      sig0)))
 
-  (** val tc1 : PrimUntyped.ufn1 -> type0 -> (PrimTyped.fn1, fn_tc_error) result **)
+  (** val tc1 :
+      PrimUntyped.ufn1 -> type0 -> (PrimTyped.fn1, fn_tc_error) result **)
 
   let tc1 fn tau1 =
     match fn with
@@ -950,10 +979,14 @@ module PrimTypeInference =
          Success (PrimTyped.Bits1
            (match fn0 with
             | PrimUntyped.UNot -> PrimTyped.Not (Obj.magic sz1)
-            | PrimUntyped.USExt width -> PrimTyped.SExt ((Obj.magic sz1), width)
-            | PrimUntyped.UZExtL width -> PrimTyped.ZExtL ((Obj.magic sz1), width)
-            | PrimUntyped.UZExtR width -> PrimTyped.ZExtR ((Obj.magic sz1), width)
-            | PrimUntyped.URepeat times -> PrimTyped.Repeat ((Obj.magic sz1), times)
+            | PrimUntyped.USExt width ->
+              PrimTyped.SExt ((Obj.magic sz1), width)
+            | PrimUntyped.UZExtL width ->
+              PrimTyped.ZExtL ((Obj.magic sz1), width)
+            | PrimUntyped.UZExtR width ->
+              PrimTyped.ZExtR ((Obj.magic sz1), width)
+            | PrimUntyped.URepeat times ->
+              PrimTyped.Repeat ((Obj.magic sz1), times)
             | PrimUntyped.USlice (offset, width) ->
               PrimTyped.Slice ((Obj.magic sz1), offset, width)))
        | Failure f -> Failure f)
@@ -963,7 +996,8 @@ module PrimTypeInference =
          (match assert_kind (Kind_struct None) Arg1 tau1 with
           | Success sig0 ->
             (match find_field (Obj.magic sig0) f with
-             | Success idx -> Success (PrimTyped.Struct1 ((Obj.magic sig0), idx))
+             | Success idx ->
+               Success (PrimTyped.Struct1 ((Obj.magic sig0), idx))
              | Failure f0 -> Failure f0)
           | Failure f0 -> Failure f0)
        | PrimUntyped.UGetFieldBits (sig0, f) ->
@@ -977,7 +1011,8 @@ module PrimTypeInference =
          (match assert_kind (Kind_array None) Arg1 tau1 with
           | Success sig0 ->
             (match check_index (Obj.magic sig0) pos with
-             | Success idx -> Success (PrimTyped.Array1 ((Obj.magic sig0), idx))
+             | Success idx ->
+               Success (PrimTyped.Array1 ((Obj.magic sig0), idx))
              | Failure f -> Failure f)
           | Failure f -> Failure f)
        | PrimUntyped.UGetElementBits (sig0, pos) ->
@@ -987,7 +1022,8 @@ module PrimTypeInference =
           | Failure f -> Failure f))
 
   (** val tc2 :
-      PrimUntyped.ufn2 -> type0 -> type0 -> (PrimTyped.fn2, fn_tc_error) result **)
+      PrimUntyped.ufn2 -> type0 -> type0 -> (PrimTyped.fn2, fn_tc_error)
+      result **)
 
   let tc2 fn tau1 tau2 =
     match fn with
@@ -1002,9 +1038,12 @@ module PrimTypeInference =
                | PrimUntyped.UAnd -> PrimTyped.And (Obj.magic sz1)
                | PrimUntyped.UOr -> PrimTyped.Or (Obj.magic sz1)
                | PrimUntyped.UXor -> PrimTyped.Xor (Obj.magic sz1)
-               | PrimUntyped.ULsl -> PrimTyped.Lsl ((Obj.magic sz1), (Obj.magic sz2))
-               | PrimUntyped.ULsr -> PrimTyped.Lsr ((Obj.magic sz1), (Obj.magic sz2))
-               | PrimUntyped.UAsr -> PrimTyped.Asr ((Obj.magic sz1), (Obj.magic sz2))
+               | PrimUntyped.ULsl ->
+                 PrimTyped.Lsl ((Obj.magic sz1), (Obj.magic sz2))
+               | PrimUntyped.ULsr ->
+                 PrimTyped.Lsr ((Obj.magic sz1), (Obj.magic sz2))
+               | PrimUntyped.UAsr ->
+                 PrimTyped.Asr ((Obj.magic sz1), (Obj.magic sz2))
                | PrimUntyped.UConcat ->
                  PrimTyped.Concat ((Obj.magic sz1), (Obj.magic sz2))
                | PrimUntyped.USel -> PrimTyped.Sel (Obj.magic sz1)
@@ -1014,7 +1053,8 @@ module PrimTypeInference =
                  PrimTyped.IndexedSlice ((Obj.magic sz1), width)
                | PrimUntyped.UPlus -> PrimTyped.Plus (Obj.magic sz1)
                | PrimUntyped.UMinus -> PrimTyped.Minus (Obj.magic sz1)
-               | PrimUntyped.UMul -> PrimTyped.Mul ((Obj.magic sz1), (Obj.magic sz2))
+               | PrimUntyped.UMul ->
+                 PrimTyped.Mul ((Obj.magic sz1), (Obj.magic sz2))
                | PrimUntyped.UCompare (signed, c) ->
                  PrimTyped.Compare (signed, c, (Obj.magic sz1))))
           | Failure f -> Failure f)
@@ -1025,7 +1065,8 @@ module PrimTypeInference =
          (match assert_kind (Kind_struct None) Arg1 tau1 with
           | Success sig0 ->
             (match find_field (Obj.magic sig0) f with
-             | Success idx -> Success (PrimTyped.Struct2 ((Obj.magic sig0), idx))
+             | Success idx ->
+               Success (PrimTyped.Struct2 ((Obj.magic sig0), idx))
              | Failure f0 -> Failure f0)
           | Failure f0 -> Failure f0)
        | PrimUntyped.USubstFieldBits (sig0, f) ->
@@ -1039,13 +1080,15 @@ module PrimTypeInference =
          (match assert_kind (Kind_array None) Arg1 tau1 with
           | Success sig0 ->
             (match check_index (Obj.magic sig0) pos with
-             | Success idx -> Success (PrimTyped.Array2 ((Obj.magic sig0), idx))
+             | Success idx ->
+               Success (PrimTyped.Array2 ((Obj.magic sig0), idx))
              | Failure f -> Failure f)
           | Failure f -> Failure f)
        | PrimUntyped.USubstElementBits (sig0, pos) ->
          (match check_index sig0 pos with
           | Success idx ->
-            Success (PrimTyped.Bits2 (PrimTyped.coq_SubstElementBits sig0 idx))
+            Success (PrimTyped.Bits2
+              (PrimTyped.coq_SubstElementBits sig0 idx))
           | Failure f -> Failure f))
  end
 
@@ -1059,21 +1102,26 @@ module CircuitSignatures =
         (match fn with
          | PrimTyped.DisplayUtf8 len ->
            Array_t { array_type = (Bits_t (Stdlib.Int.succ (Stdlib.Int.succ
-             (Stdlib.Int.succ (Stdlib.Int.succ (Stdlib.Int.succ (Stdlib.Int.succ
-             (Stdlib.Int.succ (Stdlib.Int.succ 0))))))))); array_len = len }
-         | PrimTyped.DisplayValue (tau, _) -> tau) (Obj.magic __)); retSig = (Bits_t
-      0) }
+             (Stdlib.Int.succ (Stdlib.Int.succ (Stdlib.Int.succ
+             (Stdlib.Int.succ (Stdlib.Int.succ (Stdlib.Int.succ 0)))))))));
+             array_len = len }
+         | PrimTyped.DisplayValue (tau, _) -> tau) (Obj.magic __)); retSig =
+      (Bits_t 0) }
 
   (** val coq_CSigma1 : PrimTyped.fbits1 -> int _Sig **)
 
   let coq_CSigma1 = function
-  | PrimTyped.Not sz0 -> { argSigs = (vect_cons 0 sz0 (Obj.magic __)); retSig = sz0 }
+  | PrimTyped.Not sz0 ->
+    { argSigs = (vect_cons 0 sz0 (Obj.magic __)); retSig = sz0 }
   | PrimTyped.SExt (sz0, width) ->
-    { argSigs = (vect_cons 0 sz0 (Obj.magic __)); retSig = (Nat.max sz0 width) }
+    { argSigs = (vect_cons 0 sz0 (Obj.magic __)); retSig =
+      (Nat.max sz0 width) }
   | PrimTyped.ZExtL (sz0, width) ->
-    { argSigs = (vect_cons 0 sz0 (Obj.magic __)); retSig = (Nat.max sz0 width) }
+    { argSigs = (vect_cons 0 sz0 (Obj.magic __)); retSig =
+      (Nat.max sz0 width) }
   | PrimTyped.ZExtR (sz0, width) ->
-    { argSigs = (vect_cons 0 sz0 (Obj.magic __)); retSig = (Nat.max sz0 width) }
+    { argSigs = (vect_cons 0 sz0 (Obj.magic __)); retSig =
+      (Nat.max sz0 width) }
   | PrimTyped.Repeat (sz0, times) ->
     { argSigs = (vect_cons 0 sz0 (Obj.magic __)); retSig = (mul times sz0) }
   | PrimTyped.Slice (sz0, _, width) ->
@@ -1089,55 +1137,65 @@ module CircuitSignatures =
 
   let coq_CSigma2 = function
   | PrimTyped.And sz0 ->
-    { argSigs = (vect_cons (Stdlib.Int.succ 0) sz0 (vect_cons 0 sz0 (Obj.magic __)));
+    { argSigs =
+      (vect_cons (Stdlib.Int.succ 0) sz0 (vect_cons 0 sz0 (Obj.magic __)));
       retSig = sz0 }
   | PrimTyped.Or sz0 ->
-    { argSigs = (vect_cons (Stdlib.Int.succ 0) sz0 (vect_cons 0 sz0 (Obj.magic __)));
+    { argSigs =
+      (vect_cons (Stdlib.Int.succ 0) sz0 (vect_cons 0 sz0 (Obj.magic __)));
       retSig = sz0 }
   | PrimTyped.Xor sz0 ->
-    { argSigs = (vect_cons (Stdlib.Int.succ 0) sz0 (vect_cons 0 sz0 (Obj.magic __)));
+    { argSigs =
+      (vect_cons (Stdlib.Int.succ 0) sz0 (vect_cons 0 sz0 (Obj.magic __)));
       retSig = sz0 }
   | PrimTyped.Lsl (bits_sz, shift_sz) ->
     { argSigs =
-      (vect_cons (Stdlib.Int.succ 0) bits_sz (vect_cons 0 shift_sz (Obj.magic __)));
-      retSig = bits_sz }
+      (vect_cons (Stdlib.Int.succ 0) bits_sz
+        (vect_cons 0 shift_sz (Obj.magic __))); retSig = bits_sz }
   | PrimTyped.Lsr (bits_sz, shift_sz) ->
     { argSigs =
-      (vect_cons (Stdlib.Int.succ 0) bits_sz (vect_cons 0 shift_sz (Obj.magic __)));
-      retSig = bits_sz }
+      (vect_cons (Stdlib.Int.succ 0) bits_sz
+        (vect_cons 0 shift_sz (Obj.magic __))); retSig = bits_sz }
   | PrimTyped.Asr (bits_sz, shift_sz) ->
     { argSigs =
-      (vect_cons (Stdlib.Int.succ 0) bits_sz (vect_cons 0 shift_sz (Obj.magic __)));
-      retSig = bits_sz }
+      (vect_cons (Stdlib.Int.succ 0) bits_sz
+        (vect_cons 0 shift_sz (Obj.magic __))); retSig = bits_sz }
   | PrimTyped.Concat (sz1, sz2) ->
-    { argSigs = (vect_cons (Stdlib.Int.succ 0) sz1 (vect_cons 0 sz2 (Obj.magic __)));
+    { argSigs =
+      (vect_cons (Stdlib.Int.succ 0) sz1 (vect_cons 0 sz2 (Obj.magic __)));
       retSig = (add sz2 sz1) }
   | PrimTyped.Sel sz0 ->
     { argSigs =
       (vect_cons (Stdlib.Int.succ 0) sz0
-        (vect_cons 0 (Nat.log2_up sz0) (Obj.magic __))); retSig = (Stdlib.Int.succ 0) }
+        (vect_cons 0 (Nat.log2_up sz0) (Obj.magic __))); retSig =
+      (Stdlib.Int.succ 0) }
   | PrimTyped.SliceSubst (sz0, _, width) ->
     { argSigs =
-      (vect_cons (Stdlib.Int.succ 0) sz0 (vect_cons 0 width (Obj.magic __))); retSig =
-      sz0 }
+      (vect_cons (Stdlib.Int.succ 0) sz0 (vect_cons 0 width (Obj.magic __)));
+      retSig = sz0 }
   | PrimTyped.IndexedSlice (sz0, width) ->
     { argSigs =
       (vect_cons (Stdlib.Int.succ 0) sz0
         (vect_cons 0 (Nat.log2_up sz0) (Obj.magic __))); retSig = width }
   | PrimTyped.Plus sz0 ->
-    { argSigs = (vect_cons (Stdlib.Int.succ 0) sz0 (vect_cons 0 sz0 (Obj.magic __)));
+    { argSigs =
+      (vect_cons (Stdlib.Int.succ 0) sz0 (vect_cons 0 sz0 (Obj.magic __)));
       retSig = sz0 }
   | PrimTyped.Minus sz0 ->
-    { argSigs = (vect_cons (Stdlib.Int.succ 0) sz0 (vect_cons 0 sz0 (Obj.magic __)));
+    { argSigs =
+      (vect_cons (Stdlib.Int.succ 0) sz0 (vect_cons 0 sz0 (Obj.magic __)));
       retSig = sz0 }
   | PrimTyped.Mul (sz1, sz2) ->
-    { argSigs = (vect_cons (Stdlib.Int.succ 0) sz1 (vect_cons 0 sz2 (Obj.magic __)));
+    { argSigs =
+      (vect_cons (Stdlib.Int.succ 0) sz1 (vect_cons 0 sz2 (Obj.magic __)));
       retSig = (add sz1 sz2) }
   | PrimTyped.EqBits (sz0, _) ->
-    { argSigs = (vect_cons (Stdlib.Int.succ 0) sz0 (vect_cons 0 sz0 (Obj.magic __)));
+    { argSigs =
+      (vect_cons (Stdlib.Int.succ 0) sz0 (vect_cons 0 sz0 (Obj.magic __)));
       retSig = (Stdlib.Int.succ 0) }
   | PrimTyped.Compare (_, _, sz0) ->
-    { argSigs = (vect_cons (Stdlib.Int.succ 0) sz0 (vect_cons 0 sz0 (Obj.magic __)));
+    { argSigs =
+      (vect_cons (Stdlib.Int.succ 0) sz0 (vect_cons 0 sz0 (Obj.magic __)));
       retSig = (Stdlib.Int.succ 0) }
  end
 
@@ -1150,9 +1208,11 @@ module PrimSignatures =
   | PrimTyped.Conv (tau, fn0) ->
     (match fn0 with
      | PrimTyped.Pack ->
-       { argSigs = (vect_cons 0 tau (Obj.magic __)); retSig = (Bits_t (type_sz tau)) }
+       { argSigs = (vect_cons 0 tau (Obj.magic __)); retSig = (Bits_t
+         (type_sz tau)) }
      | PrimTyped.Unpack ->
-       { argSigs = (vect_cons 0 (Bits_t (type_sz tau)) (Obj.magic __)); retSig = tau }
+       { argSigs = (vect_cons 0 (Bits_t (type_sz tau)) (Obj.magic __));
+         retSig = tau }
      | PrimTyped.Ignore ->
        { argSigs = (vect_cons 0 tau (Obj.magic __)); retSig = (Bits_t 0) })
   | PrimTyped.Bits1 fn0 ->
@@ -1161,13 +1221,15 @@ module PrimSignatures =
     { argSigs = (vect_cons 0 (Struct_t sig0) (Obj.magic __)); retSig =
       (field_type sig0 idx) }
   | PrimTyped.Array1 (sig0, _) ->
-    { argSigs = (vect_cons 0 (Array_t sig0) (Obj.magic __)); retSig = sig0.array_type }
+    { argSigs = (vect_cons 0 (Array_t sig0) (Obj.magic __)); retSig =
+      sig0.array_type }
 
   (** val coq_Sigma2 : PrimTyped.fn2 -> type0 _Sig **)
 
   let coq_Sigma2 = function
   | PrimTyped.Eq (tau, _) ->
-    { argSigs = (vect_cons (Stdlib.Int.succ 0) tau (vect_cons 0 tau (Obj.magic __)));
+    { argSigs =
+      (vect_cons (Stdlib.Int.succ 0) tau (vect_cons 0 tau (Obj.magic __)));
       retSig = (Bits_t (Stdlib.Int.succ 0)) }
   | PrimTyped.Bits2 fn0 ->
     sig_of_CSig (Stdlib.Int.succ (Stdlib.Int.succ 0))
@@ -1175,11 +1237,13 @@ module PrimSignatures =
   | PrimTyped.Struct2 (sig0, idx) ->
     { argSigs =
       (vect_cons (Stdlib.Int.succ 0) (Struct_t sig0)
-        (vect_cons 0 (field_type sig0 idx) (Obj.magic __))); retSig = (Struct_t sig0) }
+        (vect_cons 0 (field_type sig0 idx) (Obj.magic __))); retSig =
+      (Struct_t sig0) }
   | PrimTyped.Array2 (sig0, _) ->
     { argSigs =
       (vect_cons (Stdlib.Int.succ 0) (Array_t sig0)
-        (vect_cons 0 sig0.array_type (Obj.magic __))); retSig = (Array_t sig0) }
+        (vect_cons 0 sig0.array_type (Obj.magic __))); retSig = (Array_t
+      sig0) }
  end
 
 type ('from, 'to0) lift = 'from -> 'to0
@@ -1198,11 +1262,15 @@ type ('pos_t, 'var_t, 'fn_name_t, 'reg_t, 'ext_fn_t) uaction =
    * ('pos_t, 'var_t, 'fn_name_t, 'reg_t, 'ext_fn_t) uaction
    * ('pos_t, 'var_t, 'fn_name_t, 'reg_t, 'ext_fn_t) uaction
 | URead of port * 'reg_t
-| UWrite of port * 'reg_t * ('pos_t, 'var_t, 'fn_name_t, 'reg_t, 'ext_fn_t) uaction
-| UUnop of PrimUntyped.ufn1 * ('pos_t, 'var_t, 'fn_name_t, 'reg_t, 'ext_fn_t) uaction
-| UBinop of PrimUntyped.ufn2 * ('pos_t, 'var_t, 'fn_name_t, 'reg_t, 'ext_fn_t) uaction
+| UWrite of port * 'reg_t
    * ('pos_t, 'var_t, 'fn_name_t, 'reg_t, 'ext_fn_t) uaction
-| UExternalCall of 'ext_fn_t * ('pos_t, 'var_t, 'fn_name_t, 'reg_t, 'ext_fn_t) uaction
+| UUnop of PrimUntyped.ufn1
+   * ('pos_t, 'var_t, 'fn_name_t, 'reg_t, 'ext_fn_t) uaction
+| UBinop of PrimUntyped.ufn2
+   * ('pos_t, 'var_t, 'fn_name_t, 'reg_t, 'ext_fn_t) uaction
+   * ('pos_t, 'var_t, 'fn_name_t, 'reg_t, 'ext_fn_t) uaction
+| UExternalCall of 'ext_fn_t
+   * ('pos_t, 'var_t, 'fn_name_t, 'reg_t, 'ext_fn_t) uaction
 | UInternalCall of ('var_t, 'fn_name_t, ('pos_t, 'var_t, 'fn_name_t, 'reg_t,
                    'ext_fn_t) uaction) internalFunction
    * ('pos_t, 'var_t, 'fn_name_t, 'reg_t, 'ext_fn_t) uaction list
@@ -1215,20 +1283,23 @@ and ('pos_t, 'var_t, 'fn_name_t, 'reg_t, 'ext_fn_t) usugar =
 | UConstString of char list
 | UConstEnum of enum_sig * char list
 | UProgn of ('pos_t, 'var_t, 'fn_name_t, 'reg_t, 'ext_fn_t) uaction list
-| ULet of ('var_t * ('pos_t, 'var_t, 'fn_name_t, 'reg_t, 'ext_fn_t) uaction) list
-   * ('pos_t, 'var_t, 'fn_name_t, 'reg_t, 'ext_fn_t) uaction
+| ULet of ('var_t * ('pos_t, 'var_t, 'fn_name_t, 'reg_t, 'ext_fn_t) uaction)
+          list * ('pos_t, 'var_t, 'fn_name_t, 'reg_t, 'ext_fn_t) uaction
 | UWhen of ('pos_t, 'var_t, 'fn_name_t, 'reg_t, 'ext_fn_t) uaction
    * ('pos_t, 'var_t, 'fn_name_t, 'reg_t, 'ext_fn_t) uaction
 | USwitch of ('pos_t, 'var_t, 'fn_name_t, 'reg_t, 'ext_fn_t) uaction
    * ('pos_t, 'var_t, 'fn_name_t, 'reg_t, 'ext_fn_t) uaction
-   * (('pos_t, 'var_t, 'fn_name_t, 'reg_t, 'ext_fn_t) uaction * ('pos_t, 'var_t,
-     'fn_name_t, 'reg_t, 'ext_fn_t) uaction) list
+   * (('pos_t, 'var_t, 'fn_name_t, 'reg_t, 'ext_fn_t) uaction * ('pos_t,
+     'var_t, 'fn_name_t, 'reg_t, 'ext_fn_t) uaction) list
 | UStructInit of type0 struct_sig'
-   * (char list * ('pos_t, 'var_t, 'fn_name_t, 'reg_t, 'ext_fn_t) uaction) list
-| UArrayInit of type0 * ('pos_t, 'var_t, 'fn_name_t, 'reg_t, 'ext_fn_t) uaction list
+   * (char list * ('pos_t, 'var_t, 'fn_name_t, 'reg_t, 'ext_fn_t) uaction)
+     list
+| UArrayInit of type0
+   * ('pos_t, 'var_t, 'fn_name_t, 'reg_t, 'ext_fn_t) uaction list
 | UCallModule of (__ -> 'reg_t) * (__, 'ext_fn_t) lift
    * ('var_t, 'fn_name_t, ('pos_t, 'var_t, 'fn_name_t, __, __) uaction)
-     internalFunction * ('pos_t, 'var_t, 'fn_name_t, 'reg_t, 'ext_fn_t) uaction list
+     internalFunction
+   * ('pos_t, 'var_t, 'fn_name_t, 'reg_t, 'ext_fn_t) uaction list
 
 type ('pos_t, 'rule_name_t) scheduler =
 | Done
@@ -1243,12 +1314,14 @@ type ('pos_t, 'var_t, 'fn_name_t, 'reg_t, 'ext_fn_t) action =
 | Const of 'var_t tsig * type0 * type_denote
 | Assign of ('var_t * type0) list * 'var_t * type0 * ('var_t * type0) member
    * ('pos_t, 'var_t, 'fn_name_t, 'reg_t, 'ext_fn_t) action
-| Seq of 'var_t tsig * type0 * ('pos_t, 'var_t, 'fn_name_t, 'reg_t, 'ext_fn_t) action
+| Seq of 'var_t tsig * type0
+   * ('pos_t, 'var_t, 'fn_name_t, 'reg_t, 'ext_fn_t) action
    * ('pos_t, 'var_t, 'fn_name_t, 'reg_t, 'ext_fn_t) action
 | Bind of 'var_t tsig * type0 * type0 * 'var_t
    * ('pos_t, 'var_t, 'fn_name_t, 'reg_t, 'ext_fn_t) action
    * ('pos_t, 'var_t, 'fn_name_t, 'reg_t, 'ext_fn_t) action
-| If of 'var_t tsig * type0 * ('pos_t, 'var_t, 'fn_name_t, 'reg_t, 'ext_fn_t) action
+| If of 'var_t tsig * type0
+   * ('pos_t, 'var_t, 'fn_name_t, 'reg_t, 'ext_fn_t) action
    * ('pos_t, 'var_t, 'fn_name_t, 'reg_t, 'ext_fn_t) action
    * ('pos_t, 'var_t, 'fn_name_t, 'reg_t, 'ext_fn_t) action
 | Read of 'var_t tsig * port * 'reg_t
@@ -1262,8 +1335,8 @@ type ('pos_t, 'var_t, 'fn_name_t, 'reg_t, 'ext_fn_t) action =
 | ExternalCall of 'var_t tsig * 'ext_fn_t
    * ('pos_t, 'var_t, 'fn_name_t, 'reg_t, 'ext_fn_t) action
 | InternalCall of 'var_t tsig * type0 * 'fn_name_t * 'var_t tsig
-   * ('var_t * type0, ('pos_t, 'var_t, 'fn_name_t, 'reg_t, 'ext_fn_t) action) context
-   * ('pos_t, 'var_t, 'fn_name_t, 'reg_t, 'ext_fn_t) action
+   * ('var_t * type0, ('pos_t, 'var_t, 'fn_name_t, 'reg_t, 'ext_fn_t) action)
+     context * ('pos_t, 'var_t, 'fn_name_t, 'reg_t, 'ext_fn_t) action
 | APos of 'var_t tsig * type0 * 'pos_t
    * ('pos_t, 'var_t, 'fn_name_t, 'reg_t, 'ext_fn_t) action
 
@@ -1279,17 +1352,20 @@ let bits_of_ascii c =
   let h i = (n land (1 lsl i)) <> 0 in
   f (h 0) (h 1) (h 2) (h 3) (h 4) (h 5) (h 6) (h 7))
     (fun b0 b1 b2 b3 b4 b5 b6 b7 ->
-    vect_cons (Stdlib.Int.succ (Stdlib.Int.succ (Stdlib.Int.succ (Stdlib.Int.succ
-      (Stdlib.Int.succ (Stdlib.Int.succ (Stdlib.Int.succ 0))))))) b0
-      (vect_cons (Stdlib.Int.succ (Stdlib.Int.succ (Stdlib.Int.succ (Stdlib.Int.succ
-        (Stdlib.Int.succ (Stdlib.Int.succ 0)))))) b1
-        (vect_cons (Stdlib.Int.succ (Stdlib.Int.succ (Stdlib.Int.succ (Stdlib.Int.succ
-          (Stdlib.Int.succ 0))))) b2
+    vect_cons (Stdlib.Int.succ (Stdlib.Int.succ (Stdlib.Int.succ
+      (Stdlib.Int.succ (Stdlib.Int.succ (Stdlib.Int.succ (Stdlib.Int.succ
+      0))))))) b0
+      (vect_cons (Stdlib.Int.succ (Stdlib.Int.succ (Stdlib.Int.succ
+        (Stdlib.Int.succ (Stdlib.Int.succ (Stdlib.Int.succ 0)))))) b1
+        (vect_cons (Stdlib.Int.succ (Stdlib.Int.succ (Stdlib.Int.succ
+          (Stdlib.Int.succ (Stdlib.Int.succ 0))))) b2
           (vect_cons (Stdlib.Int.succ (Stdlib.Int.succ (Stdlib.Int.succ
             (Stdlib.Int.succ 0)))) b3
-            (vect_cons (Stdlib.Int.succ (Stdlib.Int.succ (Stdlib.Int.succ 0))) b4
+            (vect_cons (Stdlib.Int.succ (Stdlib.Int.succ (Stdlib.Int.succ
+              0))) b4
               (vect_cons (Stdlib.Int.succ (Stdlib.Int.succ 0)) b5
-                (vect_cons (Stdlib.Int.succ 0) b6 (vect_cons 0 b7 (Obj.magic __)))))))))
+                (vect_cons (Stdlib.Int.succ 0) b6
+                  (vect_cons 0 b7 (Obj.magic __)))))))))
     c
 
 (** val array_of_bytes : char list -> bool vect vect **)
@@ -1299,7 +1375,8 @@ let rec array_of_bytes = function
 | c::s0 -> vect_cons (length0 s0) (bits_of_ascii c) (array_of_bytes s0)
 
 (** val uprogn :
-    ('a1, 'a2, 'a3, 'a4, 'a5) uaction list -> ('a1, 'a2, 'a3, 'a4, 'a5) uaction **)
+    ('a1, 'a2, 'a3, 'a4, 'a5) uaction list -> ('a1, 'a2, 'a3, 'a4, 'a5)
+    uaction **)
 
 let rec uprogn = function
 | [] -> UConst ((Bits_t 0), (Obj.magic __))
@@ -1315,24 +1392,26 @@ let uskip =
 (** val uinit : type0 -> ('a1, 'a2, 'a3, 'a4, 'a5) uaction **)
 
 let uinit tau =
-  let zeroes = UConst ((Bits_t (type_sz tau)), (vect_const (type_sz tau) false)) in
+  let zeroes = UConst ((Bits_t (type_sz tau)),
+    (vect_const (type_sz tau) false))
+  in
   UUnop ((PrimUntyped.UConv (PrimUntyped.UUnpack tau)), zeroes)
 
 (** val ustruct_init :
-    type0 struct_sig' -> (char list * ('a1, 'a2, 'a3, 'a4, 'a5) uaction) list -> ('a1,
-    'a2, 'a3, 'a4, 'a5) uaction **)
+    type0 struct_sig' -> (char list * ('a1, 'a2, 'a3, 'a4, 'a5) uaction) list
+    -> ('a1, 'a2, 'a3, 'a4, 'a5) uaction **)
 
 let ustruct_init sig0 fields =
   let empty = uinit (Struct_t sig0) in
-  let usubst = fun f x x0 -> UBinop ((PrimUntyped.UStruct2 (PrimUntyped.USubstField
-    f)), x, x0)
+  let usubst = fun f x x0 -> UBinop ((PrimUntyped.UStruct2
+    (PrimUntyped.USubstField f)), x, x0)
   in
   fold_left (fun acc pat -> let (f, a) = pat in usubst f acc a) fields empty
 
 (** val uswitch :
-    ('a1, 'a2, 'a3, 'a4, 'a5) uaction -> ('a1, 'a2, 'a3, 'a4, 'a5) uaction -> (('a1,
-    'a2, 'a3, 'a4, 'a5) uaction * ('a1, 'a2, 'a3, 'a4, 'a5) uaction) list -> ('a1,
-    'a2, 'a3, 'a4, 'a5) uaction **)
+    ('a1, 'a2, 'a3, 'a4, 'a5) uaction -> ('a1, 'a2, 'a3, 'a4, 'a5) uaction ->
+    (('a1, 'a2, 'a3, 'a4, 'a5) uaction * ('a1, 'a2, 'a3, 'a4, 'a5) uaction)
+    list -> ('a1, 'a2, 'a3, 'a4, 'a5) uaction **)
 
 let rec uswitch var default = function
 | [] -> default
@@ -1342,8 +1421,8 @@ let rec uswitch var default = function
   (uswitch var default branches0))
 
 (** val desugar_action' :
-    'a1 -> ('a6 -> 'a4) -> ('a7 -> 'a5) -> ('a1, 'a2, 'a3, 'a6, 'a7) uaction -> ('a1,
-    'a2, 'a3, 'a4, 'a5) uaction **)
+    'a1 -> ('a6 -> 'a4) -> ('a7 -> 'a5) -> ('a1, 'a2, 'a3, 'a6, 'a7) uaction
+    -> ('a1, 'a2, 'a3, 'a4, 'a5) uaction **)
 
 let desugar_action' =
   let rec desugar_action'0 pos fR fSigma a =
@@ -1356,13 +1435,15 @@ let desugar_action' =
      | UAssign (v, ex) -> UAssign (v, (d ex))
      | USeq (a1, a2) -> USeq ((d a1), (d a2))
      | UBind (v, ex, body) -> UBind (v, (d ex), (d body))
-     | UIf (cond, tbranch, fbranch) -> UIf ((d cond), (d tbranch), (d fbranch))
+     | UIf (cond, tbranch, fbranch) ->
+       UIf ((d cond), (d tbranch), (d fbranch))
      | URead (port0, idx) -> URead (port0, (fR idx))
      | UWrite (port0, idx, value) -> UWrite (port0, (fR idx), (d value))
      | UUnop (fn, arg) -> UUnop (fn, (d arg))
      | UBinop (fn, arg1, arg2) -> UBinop (fn, (d arg1), (d arg2))
      | UExternalCall (fn, arg) -> UExternalCall ((fSigma fn), (d arg))
-     | UInternalCall (fn, args) -> UInternalCall ((map_intf_body d fn), (map d args))
+     | UInternalCall (fn, args) ->
+       UInternalCall ((map_intf_body d fn), (map d args))
      | UAPos (p, e) -> UAPos (p, (d e))
      | USugar s -> desugar __ __ pos fR fSigma s)
   and desugar _ _ pos fR fSigma s =
@@ -1372,23 +1453,26 @@ let desugar_action' =
      | USkip -> uskip
      | UConstBits (sz0, bs) -> UConst ((Bits_t sz0), bs)
      | UConstString s0 ->
-       UConst ((Array_t { array_type = (Bits_t (Stdlib.Int.succ (Stdlib.Int.succ
+       UConst ((Array_t { array_type = (Bits_t (Stdlib.Int.succ
          (Stdlib.Int.succ (Stdlib.Int.succ (Stdlib.Int.succ (Stdlib.Int.succ
-         (Stdlib.Int.succ (Stdlib.Int.succ 0))))))))); array_len = (length0 s0) }),
-         (array_of_bytes s0))
+         (Stdlib.Int.succ (Stdlib.Int.succ (Stdlib.Int.succ 0)))))))));
+         array_len = (length0 s0) }), (array_of_bytes s0))
      | UConstEnum (sig0, name) ->
        (match vect_index sig0.enum_size eqDec_string name sig0.enum_members with
         | Some idx ->
-          UConst ((Enum_t sig0), (vect_nth sig0.enum_size sig0.enum_bitpatterns idx))
-        | None -> UError { epos = pos; emsg = (UnboundEnumMember (name, sig0)) })
+          UConst ((Enum_t sig0),
+            (vect_nth sig0.enum_size sig0.enum_bitpatterns idx))
+        | None ->
+          UError { epos = pos; emsg = (UnboundEnumMember (name, sig0)) })
      | UProgn aa -> uprogn (map d aa)
      | ULet (bindings, body) ->
-       fold_right (fun pat acc -> let (var, a) = pat in UBind (var, (d a), acc))
-         (d body) bindings
+       fold_right (fun pat acc ->
+         let (var, a) = pat in UBind (var, (d a), acc)) (d body) bindings
      | UWhen (cond, body) -> UIf ((d cond), (d body), (UFail (Bits_t 0)))
      | USwitch (var, default, branches) ->
        let branches0 =
-         map (fun pat -> let (cond, body) = pat in ((d cond), (d body))) branches
+         map (fun pat -> let (cond, body) = pat in ((d cond), (d body)))
+           branches
        in
        uswitch (d var) (d default) branches0
      | UStructInit (sig0, fields) ->
@@ -1402,8 +1486,9 @@ let desugar_action' =
        let empty = uinit (Array_t sig0) in
        snd
          (fold_left (fun pat a ->
-           let (pos0, acc) = pat in ((Stdlib.Int.succ pos0), (usubst pos0 acc (d a))))
-           elements (0, empty))
+           let (pos0, acc) = pat in
+           ((Stdlib.Int.succ pos0), (usubst pos0 acc (d a)))) elements (0,
+           empty))
      | UCallModule (fR', fSigma', fn, args) ->
        let df = fun body ->
          Obj.magic desugar_action'0 pos (fun r0 -> fR (fR' r0)) (fun fn0 ->
@@ -1413,31 +1498,35 @@ let desugar_action' =
   in desugar_action'0
 
 (** val desugar_action :
-    'a1 -> ('a1, 'a2, 'a3, 'a4, 'a5) uaction -> ('a1, 'a2, 'a3, 'a4, 'a5) uaction **)
+    'a1 -> ('a1, 'a2, 'a3, 'a4, 'a5) uaction -> ('a1, 'a2, 'a3, 'a4, 'a5)
+    uaction **)
 
 let desugar_action pos a =
   desugar_action' pos (fun r0 -> r0) (fun fn -> fn) a
 
 (** val lift_basic_error_message :
-    ('a4 -> type0) -> ('a5 -> externalSignature) -> 'a1 -> 'a2 tsig -> type0 -> ('a1,
-    'a2, 'a3, 'a4, 'a5) action -> basic_error_message -> ('a1, 'a2, 'a3) error **)
+    ('a4 -> type0) -> ('a5 -> externalSignature) -> 'a1 -> 'a2 tsig -> type0
+    -> ('a1, 'a2, 'a3, 'a4, 'a5) action -> basic_error_message -> ('a1, 'a2,
+    'a3) error **)
 
 let lift_basic_error_message _ _ pos _ _ _ err =
   { epos = pos; emsg = (BasicError err) }
 
 (** val lift_fn1_tc_result :
-    ('a4 -> type0) -> ('a5 -> externalSignature) -> 'a2 tsig -> type0 -> 'a1 -> ('a1,
-    'a2, 'a3, 'a4, 'a5) action -> ('a6, fn_tc_error) result -> ('a6, ('a1, 'a2, 'a3)
-    error) result **)
+    ('a4 -> type0) -> ('a5 -> externalSignature) -> 'a2 tsig -> type0 -> 'a1
+    -> ('a1, 'a2, 'a3, 'a4, 'a5) action -> ('a6, fn_tc_error) result -> ('a6,
+    ('a1, 'a2, 'a3) error) result **)
 
 let lift_fn1_tc_result r0 sigma sig0 tau pos e r1 =
   result_map_failure (fun pat ->
-    let (_, err) = pat in lift_basic_error_message r0 sigma pos sig0 tau e err) r1
+    let (_, err) = pat in lift_basic_error_message r0 sigma pos sig0 tau e err)
+    r1
 
 (** val lift_fn2_tc_result :
-    ('a4 -> type0) -> ('a5 -> externalSignature) -> 'a2 tsig -> type0 -> 'a2 tsig ->
-    type0 -> 'a1 -> ('a1, 'a2, 'a3, 'a4, 'a5) action -> 'a1 -> ('a1, 'a2, 'a3, 'a4,
-    'a5) action -> ('a6, fn_tc_error) result -> ('a6, ('a1, 'a2, 'a3) error) result **)
+    ('a4 -> type0) -> ('a5 -> externalSignature) -> 'a2 tsig -> type0 -> 'a2
+    tsig -> type0 -> 'a1 -> ('a1, 'a2, 'a3, 'a4, 'a5) action -> 'a1 -> ('a1,
+    'a2, 'a3, 'a4, 'a5) action -> ('a6, fn_tc_error) result -> ('a6, ('a1,
+    'a2, 'a3) error) result **)
 
 let lift_fn2_tc_result r0 sigma sig1 tau1 sig2 tau2 pos1 e1 pos2 e2 r1 =
   result_map_failure (fun pat ->
@@ -1446,27 +1535,29 @@ let lift_fn2_tc_result r0 sigma sig1 tau1 sig2 tau2 pos1 e1 pos2 e2 r1 =
      | Arg1 -> lift_basic_error_message r0 sigma pos1 sig1 tau1 e1 err
      | Arg2 -> lift_basic_error_message r0 sigma pos2 sig2 tau2 e2 err)) r1
 
-(** val mkerror : 'a1 -> ('a3, 'a2) error_message -> 'a4 -> ('a1, 'a3, 'a2) error **)
+(** val mkerror :
+    'a1 -> ('a3, 'a2) error_message -> 'a4 -> ('a1, 'a3, 'a2) error **)
 
 let mkerror pos msg _ =
   { epos = pos; emsg = msg }
 
 (** val cast_action' :
-    ('a4 -> type0) -> ('a5 -> externalSignature) -> 'a1 -> 'a3 tsig -> type0 -> type0
-    -> ('a1, 'a3, 'a2, 'a4, 'a5) action -> ('a3, 'a2) error_message -> (('a1, 'a3,
-    'a2, 'a4, 'a5) action, ('a1, 'a3, 'a2) error) result **)
+    ('a4 -> type0) -> ('a5 -> externalSignature) -> 'a1 -> 'a3 tsig -> type0
+    -> type0 -> ('a1, 'a3, 'a2, 'a4, 'a5) action -> ('a3, 'a2) error_message
+    -> (('a1, 'a3, 'a2, 'a4, 'a5) action, ('a1, 'a3, 'a2) error) result **)
 
 let cast_action' _ _ pos _ tau1 tau2 e emsg0 =
   let s = eqDec_type.eq_dec tau1 tau2 in
   if s then Success e else Failure (mkerror pos emsg0 e)
 
 (** val cast_action :
-    ('a4 -> type0) -> ('a5 -> externalSignature) -> 'a1 -> 'a3 tsig -> type0 -> type0
-    -> ('a1, 'a3, 'a2, 'a4, 'a5) action -> (('a1, 'a3, 'a2, 'a4, 'a5) action, ('a1,
-    'a3, 'a2) error) result **)
+    ('a4 -> type0) -> ('a5 -> externalSignature) -> 'a1 -> 'a3 tsig -> type0
+    -> type0 -> ('a1, 'a3, 'a2, 'a4, 'a5) action -> (('a1, 'a3, 'a2, 'a4,
+    'a5) action, ('a1, 'a3, 'a2) error) result **)
 
 let cast_action r0 sigma pos sig0 tau1 tau2 e =
-  cast_action' r0 sigma pos sig0 tau1 tau2 e (BasicError (TypeMismatch (tau1, tau2)))
+  cast_action' r0 sigma pos sig0 tau1 tau2 e (BasicError (TypeMismatch (tau1,
+    tau2)))
 
 (** val actpos : 'a1 -> ('a1, 'a3, 'a2, 'a4, 'a5) uaction -> 'a1 **)
 
@@ -1475,10 +1566,10 @@ let actpos pos = function
 | _ -> pos
 
 (** val assert_argtypes' :
-    ('a4 -> type0) -> ('a5 -> externalSignature) -> 'a3 tsig -> 'a6 -> int -> 'a2 ->
-    'a1 -> 'a3 tsig -> ('a1 * (type0, ('a1, 'a3, 'a2, 'a4, 'a5) action) sigT) list ->
-    (('a3 * type0, ('a1, 'a3, 'a2, 'a4, 'a5) action) context, ('a1, 'a3, 'a2) error)
-    result **)
+    ('a4 -> type0) -> ('a5 -> externalSignature) -> 'a3 tsig -> 'a6 -> int ->
+    'a2 -> 'a1 -> 'a3 tsig -> ('a1 * (type0, ('a1, 'a3, 'a2, 'a4, 'a5)
+    action) sigT) list -> (('a3 * type0, ('a1, 'a3, 'a2, 'a4, 'a5) action)
+    context, ('a1, 'a3, 'a2) error) result **)
 
 let rec assert_argtypes' r0 sigma sig0 src nexpected fn_name pos args_desc args =
   match args_desc with
@@ -1486,53 +1577,61 @@ let rec assert_argtypes' r0 sigma sig0 src nexpected fn_name pos args_desc args 
     (match args with
      | [] -> Success CtxEmpty
      | _ :: _ ->
-       Failure (mkerror pos (TooManyArguments (fn_name, nexpected, (length args))) src))
+       Failure
+         (mkerror pos (TooManyArguments (fn_name, nexpected, (length args)))
+           src))
   | p :: fn_sig ->
     let (name1, tau1) = p in
     (match args with
      | [] ->
        Failure
-         (mkerror pos (TooFewArguments (fn_name, nexpected, (length args_desc))) src)
+         (mkerror pos (TooFewArguments (fn_name, nexpected,
+           (length args_desc))) src)
      | p0 :: args0 ->
        let (pos1, arg1) = p0 in
        (match cast_action r0 sigma pos1 sig0 (projT1 arg1) tau1 (projT2 arg1) with
         | Success arg2 ->
-          (match assert_argtypes' r0 sigma sig0 src nexpected fn_name pos fn_sig args0 with
-           | Success ctx -> Success (CtxCons (fn_sig, (name1, tau1), arg2, ctx))
+          (match assert_argtypes' r0 sigma sig0 src nexpected fn_name pos
+                   fn_sig args0 with
+           | Success ctx ->
+             Success (CtxCons (fn_sig, (name1, tau1), arg2, ctx))
            | Failure f -> Failure f)
         | Failure f -> Failure f))
 
 (** val assert_argtypes :
-    ('a4 -> type0) -> ('a5 -> externalSignature) -> 'a3 tsig -> 'a6 -> 'a2 -> 'a1 ->
-    'a3 tsig -> ('a1 * (type0, ('a1, 'a3, 'a2, 'a4, 'a5) action) sigT) list ->
-    (('a3 * type0, ('a1, 'a3, 'a2, 'a4, 'a5) action) context, ('a1, 'a3, 'a2) error)
-    result **)
+    ('a4 -> type0) -> ('a5 -> externalSignature) -> 'a3 tsig -> 'a6 -> 'a2 ->
+    'a1 -> 'a3 tsig -> ('a1 * (type0, ('a1, 'a3, 'a2, 'a4, 'a5) action) sigT)
+    list -> (('a3 * type0, ('a1, 'a3, 'a2, 'a4, 'a5) action) context, ('a1,
+    'a3, 'a2) error) result **)
 
 let assert_argtypes r0 sigma sig0 src fn_name pos args_desc args =
-  assert_argtypes' r0 sigma sig0 src (length args_desc) fn_name pos args_desc args
+  assert_argtypes' r0 sigma sig0 src (length args_desc) fn_name pos args_desc
+    args
 
 (** val type_action :
-    'a3 eqDec -> ('a4 -> type0) -> ('a5 -> externalSignature) -> 'a1 -> 'a3 tsig ->
-    ('a1, 'a3, 'a2, 'a4, 'a5) uaction -> ((type0, ('a1, 'a3, 'a2, 'a4, 'a5) action)
-    sigT, ('a1, 'a3, 'a2) error) result **)
+    'a3 eqDec -> ('a4 -> type0) -> ('a5 -> externalSignature) -> 'a1 -> 'a3
+    tsig -> ('a1, 'a3, 'a2, 'a4, 'a5) uaction -> ((type0, ('a1, 'a3, 'a2,
+    'a4, 'a5) action) sigT, ('a1, 'a3, 'a2) error) result **)
 
 let rec type_action var_t_eq_dec r0 sigma pos sig0 e = match e with
 | UError err -> Failure err
 | UFail tau -> Success (ExistT (tau, (Fail (sig0, tau))))
 | UVar var ->
-  (match opt_result (assoc var_t_eq_dec var sig0) (mkerror pos (UnboundVariable var) e) with
+  (match opt_result (assoc var_t_eq_dec var sig0)
+           (mkerror pos (UnboundVariable var) e) with
    | Success tau_m ->
      Success (ExistT ((projT1 tau_m), (Var (sig0, var, (projT1 tau_m),
        (projT2 tau_m)))))
    | Failure f -> Failure f)
 | UConst (tau, cst) -> Success (ExistT (tau, (Const (sig0, tau, cst))))
 | UAssign (var, ex) ->
-  (match opt_result (assoc var_t_eq_dec var sig0) (mkerror pos (UnboundVariable var) e) with
+  (match opt_result (assoc var_t_eq_dec var sig0)
+           (mkerror pos (UnboundVariable var) e) with
    | Success tau_m ->
      (match type_action var_t_eq_dec r0 sigma pos sig0 ex with
       | Success ex' ->
-        (match cast_action r0 sigma (actpos pos ex) sig0 (projT1 ex') (projT1 tau_m)
-                 (projT2 ex') with
+        (match cast_action r0 sigma (actpos pos ex) sig0 (projT1 ex')
+                 (projT1 tau_m) (projT2 ex') with
          | Success ex'0 ->
            Success (ExistT ((Bits_t 0), (Assign (sig0, var, (projT1 tau_m),
              (projT2 tau_m), ex'0))))
@@ -1555,27 +1654,28 @@ let rec type_action var_t_eq_dec r0 sigma pos sig0 e = match e with
 | UBind (v, ex, body) ->
   (match type_action var_t_eq_dec r0 sigma pos sig0 ex with
    | Success ex0 ->
-     (match type_action var_t_eq_dec r0 sigma pos ((v, (projT1 ex0)) :: sig0) body with
+     (match type_action var_t_eq_dec r0 sigma pos ((v, (projT1 ex0)) :: sig0)
+              body with
       | Success body0 ->
-        Success (ExistT ((projT1 body0), (Bind (sig0, (projT1 ex0), (projT1 body0), v,
-          (projT2 ex0), (projT2 body0)))))
+        Success (ExistT ((projT1 body0), (Bind (sig0, (projT1 ex0),
+          (projT1 body0), v, (projT2 ex0), (projT2 body0)))))
       | Failure f -> Failure f)
    | Failure f -> Failure f)
 | UIf (cond, tbranch, fbranch) ->
   (match type_action var_t_eq_dec r0 sigma pos sig0 cond with
    | Success cond' ->
-     (match cast_action r0 sigma (actpos pos cond) sig0 (projT1 cond') (Bits_t
-              (Stdlib.Int.succ 0)) (projT2 cond') with
+     (match cast_action r0 sigma (actpos pos cond) sig0 (projT1 cond')
+              (Bits_t (Stdlib.Int.succ 0)) (projT2 cond') with
       | Success cond'0 ->
         (match type_action var_t_eq_dec r0 sigma pos sig0 tbranch with
          | Success tbranch' ->
            (match type_action var_t_eq_dec r0 sigma pos sig0 fbranch with
             | Success fbranch' ->
-              (match cast_action r0 sigma (actpos pos fbranch) sig0 (projT1 fbranch')
-                       (projT1 tbranch') (projT2 fbranch') with
+              (match cast_action r0 sigma (actpos pos fbranch) sig0
+                       (projT1 fbranch') (projT1 tbranch') (projT2 fbranch') with
                | Success fbranch'0 ->
-                 Success (ExistT ((projT1 tbranch'), (If (sig0, (projT1 tbranch'),
-                   cond'0, (projT2 tbranch'), fbranch'0))))
+                 Success (ExistT ((projT1 tbranch'), (If (sig0,
+                   (projT1 tbranch'), cond'0, (projT2 tbranch'), fbranch'0))))
                | Failure f -> Failure f)
             | Failure f -> Failure f)
          | Failure f -> Failure f)
@@ -1585,8 +1685,8 @@ let rec type_action var_t_eq_dec r0 sigma pos sig0 e = match e with
 | UWrite (port0, idx, value) ->
   (match type_action var_t_eq_dec r0 sigma pos sig0 value with
    | Success value' ->
-     (match cast_action r0 sigma (actpos pos value) sig0 (projT1 value') (r0 idx)
-              (projT2 value') with
+     (match cast_action r0 sigma (actpos pos value) sig0 (projT1 value')
+              (r0 idx) (projT2 value') with
       | Success value'0 ->
         Success (ExistT ((Bits_t 0), (Write (sig0, port0, idx, value'0))))
       | Failure f -> Failure f)
@@ -1595,14 +1695,15 @@ let rec type_action var_t_eq_dec r0 sigma pos sig0 e = match e with
   let pos1 = actpos pos arg1 in
   (match type_action var_t_eq_dec r0 sigma pos sig0 arg1 with
    | Success arg1' ->
-     (match lift_fn1_tc_result r0 sigma sig0 (projT1 arg1') pos1 (projT2 arg1')
-              (PrimTypeInference.tc1 fn (projT1 arg1')) with
+     (match lift_fn1_tc_result r0 sigma sig0 (projT1 arg1') pos1
+              (projT2 arg1') (PrimTypeInference.tc1 fn (projT1 arg1')) with
       | Success fn0 ->
         (match cast_action r0 sigma pos1 sig0 (projT1 arg1')
-                 (vect_hd 0 (PrimSignatures.coq_Sigma1 fn0).argSigs) (projT2 arg1') with
+                 (vect_hd 0 (PrimSignatures.coq_Sigma1 fn0).argSigs)
+                 (projT2 arg1') with
          | Success arg1'0 ->
-           Success (ExistT ((PrimSignatures.coq_Sigma1 fn0).retSig, (Unop (sig0, fn0,
-             arg1'0))))
+           Success (ExistT ((PrimSignatures.coq_Sigma1 fn0).retSig, (Unop
+             (sig0, fn0, arg1'0))))
          | Failure f -> Failure f)
       | Failure f -> Failure f)
    | Failure f -> Failure f)
@@ -1613,8 +1714,8 @@ let rec type_action var_t_eq_dec r0 sigma pos sig0 e = match e with
    | Success arg1' ->
      (match type_action var_t_eq_dec r0 sigma pos sig0 arg2 with
       | Success arg2' ->
-        (match lift_fn2_tc_result r0 sigma sig0 (projT1 arg1') sig0 (projT1 arg2')
-                 pos1 (projT2 arg1') pos2 (projT2 arg2')
+        (match lift_fn2_tc_result r0 sigma sig0 (projT1 arg1') sig0
+                 (projT1 arg2') pos1 (projT2 arg1') pos2 (projT2 arg2')
                  (PrimTypeInference.tc2 fn (projT1 arg1') (projT1 arg2')) with
          | Success fn0 ->
            (match cast_action r0 sigma pos1 sig0 (projT1 arg1')
@@ -1624,10 +1725,11 @@ let rec type_action var_t_eq_dec r0 sigma pos sig0 e = match e with
               (match cast_action r0 sigma pos2 sig0 (projT1 arg2')
                        (vect_hd 0
                          (vect_tl (Stdlib.Int.succ 0)
-                           (PrimSignatures.coq_Sigma2 fn0).argSigs)) (projT2 arg2') with
+                           (PrimSignatures.coq_Sigma2 fn0).argSigs))
+                       (projT2 arg2') with
                | Success arg2'0 ->
-                 Success (ExistT ((PrimSignatures.coq_Sigma2 fn0).retSig, (Binop
-                   (sig0, fn0, arg1'0, arg2'0))))
+                 Success (ExistT ((PrimSignatures.coq_Sigma2 fn0).retSig,
+                   (Binop (sig0, fn0, arg1'0, arg2'0))))
                | Failure f -> Failure f)
             | Failure f -> Failure f)
          | Failure f -> Failure f)
@@ -1640,7 +1742,8 @@ let rec type_action var_t_eq_dec r0 sigma pos sig0 e = match e with
      (match cast_action r0 sigma pos1 sig0 (projT1 arg1')
               (vect_hd 0 (sigma fn).argSigs) (projT2 arg1') with
       | Success arg1'0 ->
-        Success (ExistT ((sigma fn).retSig, (ExternalCall (sig0, fn, arg1'0))))
+        Success (ExistT ((sigma fn).retSig, (ExternalCall (sig0, fn,
+          arg1'0))))
       | Failure f -> Failure f)
    | Failure f -> Failure f)
 | UInternalCall (fn, args) ->
@@ -1648,17 +1751,19 @@ let rec type_action var_t_eq_dec r0 sigma pos sig0 e = match e with
    | Success tc_args ->
      let arg_positions = map (actpos pos) args in
      let tc_args_w_pos = combine arg_positions tc_args in
-     (match assert_argtypes r0 sigma sig0 e fn.int_name pos (rev fn.int_argspec)
-              (rev tc_args_w_pos) with
+     (match assert_argtypes r0 sigma sig0 e fn.int_name pos
+              (rev fn.int_argspec) (rev tc_args_w_pos) with
       | Success args_ctx ->
         (match type_action var_t_eq_dec r0 sigma (actpos pos fn.int_body)
                  (rev fn.int_argspec) fn.int_body with
          | Success fn_body' ->
-           (match cast_action r0 sigma (actpos pos fn.int_body) (rev fn.int_argspec)
-                    (projT1 fn_body') fn.int_retSig (projT2 fn_body') with
+           (match cast_action r0 sigma (actpos pos fn.int_body)
+                    (rev fn.int_argspec) (projT1 fn_body') fn.int_retSig
+                    (projT2 fn_body') with
             | Success fn_body'0 ->
-              Success (ExistT (fn.int_retSig, (InternalCall (sig0, fn.int_retSig,
-                fn.int_name, fn.int_argspec, args_ctx, fn_body'0))))
+              Success (ExistT (fn.int_retSig, (InternalCall (sig0,
+                fn.int_retSig, fn.int_name, fn.int_argspec, args_ctx,
+                fn_body'0))))
             | Failure f -> Failure f)
          | Failure f -> Failure f)
       | Failure f -> Failure f)
@@ -1666,51 +1771,49 @@ let rec type_action var_t_eq_dec r0 sigma pos sig0 e = match e with
 | UAPos (pos0, e0) ->
   (match type_action var_t_eq_dec r0 sigma pos0 sig0 e0 with
    | Success e1 ->
-     Success (ExistT ((projT1 e1), (APos (sig0, (projT1 e1), pos0, (projT2 e1)))))
+     Success (ExistT ((projT1 e1), (APos (sig0, (projT1 e1), pos0,
+       (projT2 e1)))))
    | Failure f -> Failure f)
 | USugar _ -> Failure (mkerror pos SugaredConstructorInAst e)
 
 (** val tc_action :
-    'a3 eqDec -> ('a4 -> type0) -> ('a5 -> externalSignature) -> 'a1 -> 'a3 tsig ->
-    type0 -> ('a1, 'a3, 'a2, 'a4, 'a5) uaction -> (('a1, 'a3, 'a2, 'a4, 'a5) action,
-    ('a1, 'a3, 'a2) error) result **)
+    'a3 eqDec -> ('a4 -> type0) -> ('a5 -> externalSignature) -> 'a1 -> 'a3
+    tsig -> type0 -> ('a1, 'a3, 'a2, 'a4, 'a5) uaction -> (('a1, 'a3, 'a2,
+    'a4, 'a5) action, ('a1, 'a3, 'a2) error) result **)
 
 let tc_action var_t_eq_dec r0 sigma pos sig0 expected_tau e =
   match type_action var_t_eq_dec r0 sigma pos sig0 e with
-  | Success a -> cast_action r0 sigma pos sig0 (projT1 a) expected_tau (projT2 a)
+  | Success a ->
+    cast_action r0 sigma pos sig0 (projT1 a) expected_tau (projT2 a)
   | Failure f -> Failure f
 
 type ext_fn_rtl_spec = { efr_name : char list; efr_internal : bool }
 
 type ext_fn_sim_spec = { efs_name : char list; efs_method : bool }
 
-(** val empty_Sigma : __ -> externalSignature **)
-
-let empty_Sigma _ =
-  assert false (* absurd case *)
-
-(** val empty_ext_fn_props : __ -> 'a1 **)
-
-let empty_ext_fn_props _ =
-  assert false (* absurd case *)
-
 type ('pos_t, 'var_t, 'fn_name_t, 'rule_name_t, 'reg_t, 'ext_fn_t) koika_package_t = { 
 koika_var_names : 'var_t show; koika_fn_names : 'fn_name_t show;
 koika_reg_names : 'reg_t show; koika_reg_types : ('reg_t -> type0);
-koika_reg_init : ('reg_t -> type_denote); koika_reg_finite : 'reg_t finiteType;
+koika_reg_init : ('reg_t -> type_denote);
+koika_reg_finite : 'reg_t finiteType;
 koika_ext_fn_types : ('ext_fn_t -> externalSignature);
-koika_rules : ('rule_name_t -> ('pos_t, 'var_t, 'fn_name_t, 'reg_t, 'ext_fn_t) rule);
-koika_rule_external : ('rule_name_t -> bool); koika_rule_names : 'rule_name_t show;
-koika_scheduler : ('pos_t, 'rule_name_t) scheduler; koika_module_name : char list }
+koika_rules : ('rule_name_t -> ('pos_t, 'var_t, 'fn_name_t, 'reg_t,
+              'ext_fn_t) rule); koika_rule_external : ('rule_name_t -> bool);
+koika_rule_names : 'rule_name_t show;
+koika_scheduler : ('pos_t, 'rule_name_t) scheduler;
+koika_module_name : char list }
 
-type 'ext_fn_t verilog_package_t = { vp_ext_fn_specs : ('ext_fn_t -> ext_fn_rtl_spec) }
+type 'ext_fn_t verilog_package_t = { vp_ext_fn_specs : ('ext_fn_t ->
+                                                       ext_fn_rtl_spec) }
 
-type 'ext_fn_t sim_package_t = { sp_ext_fn_specs : ('ext_fn_t -> ext_fn_sim_spec);
+type 'ext_fn_t sim_package_t = { sp_ext_fn_specs : ('ext_fn_t ->
+                                                   ext_fn_sim_spec);
                                  sp_prelude : char list option }
 
-type interop_package_t = { ip_koika : (unit, char list, char list, __, __, __)
-                                      koika_package_t;
-                           ip_verilog : __ verilog_package_t; ip_sim : __ sim_package_t }
+type interop_package_t = { ip_koika : (unit, char list, char list, __, __,
+                                      __) koika_package_t;
+                           ip_verilog : __ verilog_package_t;
+                           ip_sim : __ sim_package_t }
 
 module Backends =
  struct
@@ -1748,13 +1851,15 @@ module Types =
     { struct_name =
       ('b'::('a'::('s'::('i'::('c'::('_'::('f'::('l'::('i'::('t'::[]))))))))));
       struct_fields = ((('n'::('e'::('w'::[]))), (Bits_t (Stdlib.Int.succ
-      0))) :: ((('s'::('r'::('c'::[]))), (Bits_t (Stdlib.Int.succ (Stdlib.Int.succ
+      0))) :: ((('s'::('r'::('c'::[]))), (Bits_t (Stdlib.Int.succ
+      (Stdlib.Int.succ (Stdlib.Int.succ (Stdlib.Int.succ
+      0)))))) :: ((('t'::('r'::('g'::('_'::('y'::[]))))), (Bits_t
       (Stdlib.Int.succ (Stdlib.Int.succ
-      0)))))) :: ((('t'::('r'::('g'::('_'::('y'::[]))))), (Bits_t (Stdlib.Int.succ
-      (Stdlib.Int.succ 0)))) :: ((('t'::('r'::('g'::('_'::('x'::[]))))), (Bits_t
-      (Stdlib.Int.succ (Stdlib.Int.succ 0)))) :: ((('d'::('a'::('t'::('a'::[])))),
-      (Bits_t (Stdlib.Int.succ (Stdlib.Int.succ (Stdlib.Int.succ (Stdlib.Int.succ
-      (Stdlib.Int.succ 0))))))) :: []))))) }
+      0)))) :: ((('t'::('r'::('g'::('_'::('x'::[]))))), (Bits_t
+      (Stdlib.Int.succ (Stdlib.Int.succ
+      0)))) :: ((('d'::('a'::('t'::('a'::[])))), (Bits_t (Stdlib.Int.succ
+      (Stdlib.Int.succ (Stdlib.Int.succ (Stdlib.Int.succ (Stdlib.Int.succ
+      0))))))) :: []))))) }
 
   (** val router_address : type0 struct_sig' **)
 
@@ -1762,7 +1867,8 @@ module Types =
     { struct_name =
       ('r'::('o'::('u'::('t'::('e'::('r'::('_'::('a'::('d'::('d'::('r'::('e'::('s'::('s'::[]))))))))))))));
       struct_fields = ((('y'::[]), (Bits_t (Stdlib.Int.succ (Stdlib.Int.succ
-      0)))) :: ((('x'::[]), (Bits_t (Stdlib.Int.succ (Stdlib.Int.succ 0)))) :: [])) }
+      0)))) :: ((('x'::[]), (Bits_t (Stdlib.Int.succ (Stdlib.Int.succ
+      0)))) :: [])) }
  end
 
 module type Registers =
@@ -1773,53 +1879,103 @@ module type Registers =
 module Router =
  functor (Regs:Registers) ->
  struct
+  (** val ext_fn_t_rect : 'a1 -> 'a1 **)
+
+  let ext_fn_t_rect f =
+    f
+
+  (** val ext_fn_t_rec : 'a1 -> 'a1 **)
+
+  let ext_fn_t_rec f =
+    f
+
+  (** val coq_Sigma : __ -> externalSignature **)
+
+  let coq_Sigma _ =
+    { argSigs = (vect_cons 0 (Bits_t Types.sz) (Obj.magic __)); retSig =
+      (Bits_t Types.sz) }
+
+  (** val fnsigma : __ -> sig_denote **)
+
+  let fnsigma _ =
+    Obj.magic (fun x -> x)
+
+  (** val to_tile :
+      (var_t, fn_name_t, (pos_t, var_t, fn_name_t, Regs.reg_t, __) uaction)
+      internalFunction **)
+
+  let to_tile =
+    { int_name = ('t'::('o'::('_'::('t'::('i'::('l'::('e'::[])))))));
+      int_argspec =
+      ((prod_of_argsig { arg_name = ('v'::('a'::('l'::('u'::('e'::[])))));
+         arg_type = (Bits_t Types.sz) }) :: []); int_retSig = (Bits_t 0);
+      int_body = (UExternalCall (__, (UVar
+      ('v'::('a'::('l'::('u'::('e'::[])))))))) }
+
   (** val r_send :
-      Regs.reg_t -> (var_t, fn_name_t, (pos_t, var_t, fn_name_t, Regs.reg_t, __)
-      uaction) internalFunction **)
+      Regs.reg_t -> (var_t, fn_name_t, (pos_t, var_t, fn_name_t, Regs.reg_t,
+      __) uaction) internalFunction **)
 
   let r_send reg_name =
     { int_name = ('r'::('_'::('s'::('e'::('n'::('d'::[])))))); int_argspec =
-      ((prod_of_argsig { arg_name = ('v'::('a'::('l'::('u'::('e'::[]))))); arg_type =
-         (Bits_t Types.sz) }) :: []); int_retSig = (Bits_t 0); int_body = (UWrite (P0,
-      reg_name, (UVar ('v'::('a'::('l'::('u'::('e'::[])))))))) }
+      ((prod_of_argsig { arg_name = ('v'::('a'::('l'::('u'::('e'::[])))));
+         arg_type = (Bits_t Types.sz) }) :: []); int_retSig = (Bits_t 0);
+      int_body = (UWrite (P0, reg_name, (UVar
+      ('v'::('a'::('l'::('u'::('e'::[])))))))) }
 
   (** val r_receive :
-      Regs.reg_t -> (var_t, fn_name_t, (pos_t, var_t, fn_name_t, Regs.reg_t, __)
-      uaction) internalFunction **)
+      Regs.reg_t -> (var_t, fn_name_t, (pos_t, var_t, fn_name_t, Regs.reg_t,
+      __) uaction) internalFunction **)
 
   let r_receive reg_name =
-    { int_name = ('r'::('_'::('r'::('e'::('c'::('e'::('i'::('v'::('e'::[])))))))));
-      int_argspec = []; int_retSig = (Bits_t Types.sz); int_body = (URead (P0,
-      reg_name)) }
+    { int_name =
+      ('r'::('_'::('r'::('e'::('c'::('e'::('i'::('v'::('e'::[])))))))));
+      int_argspec = []; int_retSig = (Bits_t Types.sz); int_body = (URead
+      (P0, reg_name)) }
 
   (** val _routestart_r :
-      int -> (var_t, fn_name_t, (pos_t, var_t, fn_name_t, Regs.reg_t, __) uaction)
-      internalFunction -> (var_t, fn_name_t, (pos_t, var_t, fn_name_t, Regs.reg_t, __)
-      uaction) internalFunction -> (pos_t, var_t, fn_name_t, Regs.reg_t, __) uaction **)
+      int -> (var_t, fn_name_t, (pos_t, var_t, fn_name_t, Regs.reg_t, __)
+      uaction) internalFunction -> (var_t, fn_name_t, (pos_t, var_t,
+      fn_name_t, Regs.reg_t, __) uaction) internalFunction -> (pos_t, var_t,
+      fn_name_t, Regs.reg_t, __) uaction **)
 
   let _routestart_r r_addr2 r0_send r0_receive =
     UBind (('r'::('_'::('a'::('d'::('d'::('r'::[])))))), (USugar (UConstBits
-      ((Stdlib.Int.succ (Stdlib.Int.succ (Stdlib.Int.succ (Stdlib.Int.succ 0)))),
-      (Bits.of_nat (Stdlib.Int.succ (Stdlib.Int.succ (Stdlib.Int.succ (Stdlib.Int.succ
-        0)))) r_addr2)))), (UBind (('m'::('0'::[])), (USugar (UCallModule
-      ((Obj.magic id), (Obj.magic __), (Obj.magic r0_receive), []))), (UBind
-      (('m'::('s'::('g'::[]))), (UUnop ((PrimUntyped.UConv (PrimUntyped.UUnpack
-      (Struct_t Types.basic_flit))), (UVar ('m'::('0'::[]))))), (UBind
+      ((Stdlib.Int.succ (Stdlib.Int.succ (Stdlib.Int.succ (Stdlib.Int.succ
+      0)))),
+      (Bits.of_nat (Stdlib.Int.succ (Stdlib.Int.succ (Stdlib.Int.succ
+        (Stdlib.Int.succ 0)))) r_addr2)))), (UBind (('m'::('0'::[])), (UBinop
+      ((PrimUntyped.UBits2 PrimUntyped.UXor), (USugar (UCallModule
+      ((Obj.magic id), (Obj.magic __), (Obj.magic r0_receive), []))),
+      (UExternalCall (__, (USugar (UConstBits ((Stdlib.Int.succ
+      (Stdlib.Int.succ (Stdlib.Int.succ (Stdlib.Int.succ (Stdlib.Int.succ
+      (Stdlib.Int.succ (Stdlib.Int.succ (Stdlib.Int.succ (Stdlib.Int.succ
+      (Stdlib.Int.succ (Stdlib.Int.succ (Stdlib.Int.succ (Stdlib.Int.succ
+      (Stdlib.Int.succ 0)))))))))))))),
+      (Bits.of_N (Stdlib.Int.succ (Stdlib.Int.succ (Stdlib.Int.succ
+        (Stdlib.Int.succ (Stdlib.Int.succ (Stdlib.Int.succ (Stdlib.Int.succ
+        (Stdlib.Int.succ (Stdlib.Int.succ (Stdlib.Int.succ (Stdlib.Int.succ
+        (Stdlib.Int.succ (Stdlib.Int.succ (Stdlib.Int.succ 0)))))))))))))) 0)))))))),
+      (UBind (('m'::('s'::('g'::[]))), (UUnop ((PrimUntyped.UConv
+      (PrimUntyped.UUnpack (Struct_t Types.basic_flit))), (UVar
+      ('m'::('0'::[]))))), (UBind
       (('n'::('e'::('w'::('_'::('d'::('a'::('t'::('a'::[])))))))), (UUnop
-      ((PrimUntyped.UStruct1 (PrimUntyped.UGetField ('n'::('e'::('w'::[]))))), (UVar
-      ('m'::('s'::('g'::[])))))), (UBind (('s'::('r'::('c'::('_'::('p'::[]))))),
-      (UUnop ((PrimUntyped.UStruct1 (PrimUntyped.UGetField ('s'::('r'::('c'::[]))))),
-      (UVar ('m'::('s'::('g'::[])))))), (UIf ((UBinop ((PrimUntyped.UBits2
+      ((PrimUntyped.UStruct1 (PrimUntyped.UGetField
+      ('n'::('e'::('w'::[]))))), (UVar ('m'::('s'::('g'::[])))))), (UBind
+      (('s'::('r'::('c'::('_'::('p'::[]))))), (UUnop ((PrimUntyped.UStruct1
+      (PrimUntyped.UGetField ('s'::('r'::('c'::[]))))), (UVar
+      ('m'::('s'::('g'::[])))))), (UIf ((UBinop ((PrimUntyped.UBits2
       PrimUntyped.UAnd), (UBinop ((PrimUntyped.UEq true), (UVar
       ('s'::('r'::('c'::('_'::('p'::[])))))), (UVar
       ('r'::('_'::('a'::('d'::('d'::('r'::[]))))))))), (UVar
       ('n'::('e'::('w'::('_'::('d'::('a'::('t'::('a'::[]))))))))))), (UBind
       (('t'::('r'::('g'::('_'::('x'::[]))))), (UUnop ((PrimUntyped.UStruct1
       (PrimUntyped.UGetField ('t'::('r'::('g'::('_'::('x'::[]))))))), (UVar
-      ('m'::('s'::('g'::[])))))), (UBind (('t'::('r'::('g'::('_'::('y'::[]))))),
-      (UUnop ((PrimUntyped.UStruct1 (PrimUntyped.UGetField
-      ('t'::('r'::('g'::('_'::('y'::[]))))))), (UVar ('m'::('s'::('g'::[])))))),
-      (UBind (('s'::('r'::('c'::('_'::('x'::[]))))), (UUnop ((PrimUntyped.UStruct1
+      ('m'::('s'::('g'::[])))))), (UBind
+      (('t'::('r'::('g'::('_'::('y'::[]))))), (UUnop ((PrimUntyped.UStruct1
+      (PrimUntyped.UGetField ('t'::('r'::('g'::('_'::('y'::[]))))))), (UVar
+      ('m'::('s'::('g'::[])))))), (UBind
+      (('s'::('r'::('c'::('_'::('x'::[]))))), (UUnop ((PrimUntyped.UStruct1
       (PrimUntyped.UGetField ('x'::[]))), (UUnop ((PrimUntyped.UConv
       (PrimUntyped.UUnpack (Struct_t Types.router_address))), (UVar
       ('r'::('_'::('a'::('d'::('d'::('r'::[]))))))))))), (UBind
@@ -1829,55 +1985,81 @@ module Router =
       ('r'::('_'::('a'::('d'::('d'::('r'::[]))))))))))), (UIf ((UBinop
       ((PrimUntyped.UBits2 (PrimUntyped.UCompare (false, CGt))), (UVar
       ('t'::('r'::('g'::('_'::('x'::[])))))), (UVar
-      ('s'::('r'::('c'::('_'::('x'::[])))))))), (USugar (UCallModule ((Obj.magic id),
-      (Obj.magic __), (Obj.magic r0_send), ((UUnop ((PrimUntyped.UConv
-      PrimUntyped.UPack), (UBinop ((PrimUntyped.UStruct2 (PrimUntyped.USubstField
-      ('s'::('r'::('c'::[]))))), (UVar ('m'::('s'::('g'::[])))), (UVar
-      ('r'::('_'::('a'::('d'::('d'::('r'::[]))))))))))) :: [])))), (UIf ((UBinop
-      ((PrimUntyped.UBits2 (PrimUntyped.UCompare (false, CLt))), (UVar
-      ('t'::('r'::('g'::('_'::('x'::[])))))), (UVar
+      ('s'::('r'::('c'::('_'::('x'::[])))))))), (USugar (UCallModule
+      ((Obj.magic id), (Obj.magic __), (Obj.magic r0_send), ((UUnop
+      ((PrimUntyped.UConv PrimUntyped.UPack), (UBinop ((PrimUntyped.UStruct2
+      (PrimUntyped.USubstField ('s'::('r'::('c'::[]))))), (UVar
+      ('m'::('s'::('g'::[])))), (UVar
+      ('r'::('_'::('a'::('d'::('d'::('r'::[]))))))))))) :: [])))), (UIf
+      ((UBinop ((PrimUntyped.UBits2 (PrimUntyped.UCompare (false, CLt))),
+      (UVar ('t'::('r'::('g'::('_'::('x'::[])))))), (UVar
       ('s'::('r'::('c'::('_'::('x'::[])))))))), (UFail (Bits_t 0)), (USugar
       (UConstBits (0, (Obj.magic __)))))))))))))))), (USugar (UConstBits (0,
       (Obj.magic __)))))))))))))))
 
   (** val _routecenter_r :
-      int -> (var_t, fn_name_t, (pos_t, var_t, fn_name_t, Regs.reg_t, __) uaction)
-      internalFunction -> (var_t, fn_name_t, (pos_t, var_t, fn_name_t, Regs.reg_t, __)
-      uaction) internalFunction -> (var_t, fn_name_t, (pos_t, var_t, fn_name_t,
-      Regs.reg_t, __) uaction) internalFunction -> (var_t, fn_name_t, (pos_t, var_t,
-      fn_name_t, Regs.reg_t, __) uaction) internalFunction -> (pos_t, var_t,
-      fn_name_t, Regs.reg_t, __) uaction **)
+      int -> (var_t, fn_name_t, (pos_t, var_t, fn_name_t, Regs.reg_t, __)
+      uaction) internalFunction -> (var_t, fn_name_t, (pos_t, var_t,
+      fn_name_t, Regs.reg_t, __) uaction) internalFunction -> (var_t,
+      fn_name_t, (pos_t, var_t, fn_name_t, Regs.reg_t, __) uaction)
+      internalFunction -> (var_t, fn_name_t, (pos_t, var_t, fn_name_t,
+      Regs.reg_t, __) uaction) internalFunction -> (pos_t, var_t, fn_name_t,
+      Regs.reg_t, __) uaction **)
 
   let _routecenter_r r_addr2 r0_send r1_send r0_receive r1_receive =
     UBind (('r'::('_'::('a'::('d'::('d'::('r'::[])))))), (USugar (UConstBits
-      ((Stdlib.Int.succ (Stdlib.Int.succ (Stdlib.Int.succ (Stdlib.Int.succ 0)))),
-      (Bits.of_nat (Stdlib.Int.succ (Stdlib.Int.succ (Stdlib.Int.succ (Stdlib.Int.succ
-        0)))) r_addr2)))), (UBind (('m'::('0'::[])), (USugar (UCallModule
-      ((Obj.magic id), (Obj.magic __), (Obj.magic r0_receive), []))), (UBind
-      (('m'::('1'::[])), (USugar (UCallModule ((Obj.magic id), (Obj.magic __),
-      (Obj.magic r1_receive), []))), (UBind (('m'::('s'::('g'::[]))), (UUnop
-      ((PrimUntyped.UConv (PrimUntyped.UUnpack (Struct_t Types.basic_flit))), (UVar
+      ((Stdlib.Int.succ (Stdlib.Int.succ (Stdlib.Int.succ (Stdlib.Int.succ
+      0)))),
+      (Bits.of_nat (Stdlib.Int.succ (Stdlib.Int.succ (Stdlib.Int.succ
+        (Stdlib.Int.succ 0)))) r_addr2)))), (UBind (('m'::('0'::[])), (UBinop
+      ((PrimUntyped.UBits2 PrimUntyped.UXor), (USugar (UCallModule
+      ((Obj.magic id), (Obj.magic __), (Obj.magic r0_receive), []))),
+      (UExternalCall (__, (USugar (UConstBits ((Stdlib.Int.succ
+      (Stdlib.Int.succ (Stdlib.Int.succ (Stdlib.Int.succ (Stdlib.Int.succ
+      (Stdlib.Int.succ (Stdlib.Int.succ (Stdlib.Int.succ (Stdlib.Int.succ
+      (Stdlib.Int.succ (Stdlib.Int.succ (Stdlib.Int.succ (Stdlib.Int.succ
+      (Stdlib.Int.succ 0)))))))))))))),
+      (Bits.of_N (Stdlib.Int.succ (Stdlib.Int.succ (Stdlib.Int.succ
+        (Stdlib.Int.succ (Stdlib.Int.succ (Stdlib.Int.succ (Stdlib.Int.succ
+        (Stdlib.Int.succ (Stdlib.Int.succ (Stdlib.Int.succ (Stdlib.Int.succ
+        (Stdlib.Int.succ (Stdlib.Int.succ (Stdlib.Int.succ 0)))))))))))))) 0)))))))),
+      (UBind (('m'::('1'::[])), (UBinop ((PrimUntyped.UBits2
+      PrimUntyped.UXor), (USugar (UCallModule ((Obj.magic id),
+      (Obj.magic __), (Obj.magic r1_receive), []))), (UExternalCall (__,
+      (USugar (UConstBits ((Stdlib.Int.succ (Stdlib.Int.succ (Stdlib.Int.succ
+      (Stdlib.Int.succ (Stdlib.Int.succ (Stdlib.Int.succ (Stdlib.Int.succ
+      (Stdlib.Int.succ (Stdlib.Int.succ (Stdlib.Int.succ (Stdlib.Int.succ
+      (Stdlib.Int.succ (Stdlib.Int.succ (Stdlib.Int.succ 0)))))))))))))),
+      (Bits.of_N (Stdlib.Int.succ (Stdlib.Int.succ (Stdlib.Int.succ
+        (Stdlib.Int.succ (Stdlib.Int.succ (Stdlib.Int.succ (Stdlib.Int.succ
+        (Stdlib.Int.succ (Stdlib.Int.succ (Stdlib.Int.succ (Stdlib.Int.succ
+        (Stdlib.Int.succ (Stdlib.Int.succ (Stdlib.Int.succ 0)))))))))))))) 0)))))))),
+      (UBind (('m'::('s'::('g'::[]))), (UUnop ((PrimUntyped.UConv
+      (PrimUntyped.UUnpack (Struct_t Types.basic_flit))), (UVar
       ('m'::('0'::[]))))), (UBind
       (('n'::('e'::('w'::('_'::('d'::('a'::('t'::('a'::[])))))))), (UUnop
-      ((PrimUntyped.UStruct1 (PrimUntyped.UGetField ('n'::('e'::('w'::[]))))), (UVar
-      ('m'::('s'::('g'::[])))))), (UBind (('s'::('r'::('c'::('_'::('p'::[]))))),
-      (UUnop ((PrimUntyped.UStruct1 (PrimUntyped.UGetField ('s'::('r'::('c'::[]))))),
-      (UVar ('m'::('s'::('g'::[])))))), (USeq ((UIf ((UBinop ((PrimUntyped.UBits2
+      ((PrimUntyped.UStruct1 (PrimUntyped.UGetField
+      ('n'::('e'::('w'::[]))))), (UVar ('m'::('s'::('g'::[])))))), (UBind
+      (('s'::('r'::('c'::('_'::('p'::[]))))), (UUnop ((PrimUntyped.UStruct1
+      (PrimUntyped.UGetField ('s'::('r'::('c'::[]))))), (UVar
+      ('m'::('s'::('g'::[])))))), (USeq ((UIf ((UBinop ((PrimUntyped.UBits2
       PrimUntyped.UAnd), (UBinop ((PrimUntyped.UEq true), (UVar
       ('s'::('r'::('c'::('_'::('p'::[])))))), (UVar
       ('r'::('_'::('a'::('d'::('d'::('r'::[]))))))))), (UVar
-      ('n'::('e'::('w'::('_'::('d'::('a'::('t'::('a'::[]))))))))))), (USeq ((USugar
-      (UCallModule ((Obj.magic id), (Obj.magic __), (Obj.magic r0_send), ((UUnop
-      ((PrimUntyped.UConv PrimUntyped.UPack), (UBinop ((PrimUntyped.UStruct2
-      (PrimUntyped.USubstField ('n'::('e'::('w'::[]))))), (UVar
-      ('m'::('s'::('g'::[])))), (USugar (UConstBits ((Stdlib.Int.succ 0),
+      ('n'::('e'::('w'::('_'::('d'::('a'::('t'::('a'::[]))))))))))), (USeq
+      ((USugar (UCallModule ((Obj.magic id), (Obj.magic __),
+      (Obj.magic r0_send), ((UUnop ((PrimUntyped.UConv PrimUntyped.UPack),
+      (UBinop ((PrimUntyped.UStruct2 (PrimUntyped.USubstField
+      ('n'::('e'::('w'::[]))))), (UVar ('m'::('s'::('g'::[])))), (USugar
+      (UConstBits ((Stdlib.Int.succ 0),
       (vect_cons 0 false (Obj.magic __))))))))) :: [])))), (UBind
       (('t'::('r'::('g'::('_'::('x'::[]))))), (UUnop ((PrimUntyped.UStruct1
       (PrimUntyped.UGetField ('t'::('r'::('g'::('_'::('x'::[]))))))), (UVar
-      ('m'::('s'::('g'::[])))))), (UBind (('t'::('r'::('g'::('_'::('y'::[]))))),
-      (UUnop ((PrimUntyped.UStruct1 (PrimUntyped.UGetField
-      ('t'::('r'::('g'::('_'::('y'::[]))))))), (UVar ('m'::('s'::('g'::[])))))),
-      (UBind (('s'::('r'::('c'::('_'::('x'::[]))))), (UUnop ((PrimUntyped.UStruct1
+      ('m'::('s'::('g'::[])))))), (UBind
+      (('t'::('r'::('g'::('_'::('y'::[]))))), (UUnop ((PrimUntyped.UStruct1
+      (PrimUntyped.UGetField ('t'::('r'::('g'::('_'::('y'::[]))))))), (UVar
+      ('m'::('s'::('g'::[])))))), (UBind
+      (('s'::('r'::('c'::('_'::('x'::[]))))), (UUnop ((PrimUntyped.UStruct1
       (PrimUntyped.UGetField ('x'::[]))), (UUnop ((PrimUntyped.UConv
       (PrimUntyped.UUnpack (Struct_t Types.router_address))), (UVar
       ('r'::('_'::('a'::('d'::('d'::('r'::[]))))))))))), (UBind
@@ -1887,36 +2069,39 @@ module Router =
       ('r'::('_'::('a'::('d'::('d'::('r'::[]))))))))))), (UIf ((UBinop
       ((PrimUntyped.UBits2 (PrimUntyped.UCompare (false, CGt))), (UVar
       ('t'::('r'::('g'::('_'::('x'::[])))))), (UVar
-      ('s'::('r'::('c'::('_'::('x'::[])))))))), (USugar (UCallModule ((Obj.magic id),
-      (Obj.magic __), (Obj.magic r1_send), ((UUnop ((PrimUntyped.UConv
-      PrimUntyped.UPack), (UBinop ((PrimUntyped.UStruct2 (PrimUntyped.USubstField
-      ('s'::('r'::('c'::[]))))), (UVar ('m'::('s'::('g'::[])))), (UVar
-      ('r'::('_'::('a'::('d'::('d'::('r'::[]))))))))))) :: [])))), (UIf ((UBinop
-      ((PrimUntyped.UBits2 (PrimUntyped.UCompare (false, CLt))), (UVar
-      ('t'::('r'::('g'::('_'::('x'::[])))))), (UVar
-      ('s'::('r'::('c'::('_'::('x'::[])))))))), (USugar (UCallModule ((Obj.magic id),
-      (Obj.magic __), (Obj.magic r0_send), ((UUnop ((PrimUntyped.UConv
-      PrimUntyped.UPack), (UBinop ((PrimUntyped.UStruct2 (PrimUntyped.USubstField
-      ('s'::('r'::('c'::[]))))), (UVar ('m'::('s'::('g'::[])))), (UVar
-      ('r'::('_'::('a'::('d'::('d'::('r'::[]))))))))))) :: [])))), (USugar (UConstBits
-      (0, (Obj.magic __)))))))))))))))))), (USugar (UConstBits (0,
-      (Obj.magic __)))))), (UBind (('m'::('s'::('g'::('1'::[])))), (UUnop
-      ((PrimUntyped.UConv (PrimUntyped.UUnpack (Struct_t Types.basic_flit))), (UVar
-      ('m'::('1'::[]))))), (UBind
-      (('n'::('e'::('w'::('_'::('d'::('a'::('t'::('a'::[])))))))), (UUnop
-      ((PrimUntyped.UStruct1 (PrimUntyped.UGetField ('n'::('e'::('w'::[]))))), (UVar
-      ('m'::('s'::('g'::('1'::[]))))))), (UBind
-      (('s'::('r'::('c'::('_'::('p'::[]))))), (UUnop ((PrimUntyped.UStruct1
-      (PrimUntyped.UGetField ('s'::('r'::('c'::[]))))), (UVar
-      ('m'::('s'::('g'::('1'::[]))))))), (UIf ((UBinop ((PrimUntyped.UBits2
-      PrimUntyped.UAnd), (UBinop ((PrimUntyped.UEq true), (UVar
-      ('s'::('r'::('c'::('_'::('p'::[])))))), (UVar
-      ('r'::('_'::('a'::('d'::('d'::('r'::[]))))))))), (UVar
-      ('n'::('e'::('w'::('_'::('d'::('a'::('t'::('a'::[]))))))))))), (USeq ((USugar
-      (UCallModule ((Obj.magic id), (Obj.magic __), (Obj.magic r1_send), ((UUnop
+      ('s'::('r'::('c'::('_'::('x'::[])))))))), (USugar (UCallModule
+      ((Obj.magic id), (Obj.magic __), (Obj.magic r1_send), ((UUnop
       ((PrimUntyped.UConv PrimUntyped.UPack), (UBinop ((PrimUntyped.UStruct2
-      (PrimUntyped.USubstField ('n'::('e'::('w'::[]))))), (UVar
-      ('m'::('s'::('g'::('1'::[]))))), (USugar (UConstBits ((Stdlib.Int.succ 0),
+      (PrimUntyped.USubstField ('s'::('r'::('c'::[]))))), (UVar
+      ('m'::('s'::('g'::[])))), (UVar
+      ('r'::('_'::('a'::('d'::('d'::('r'::[]))))))))))) :: [])))), (UIf
+      ((UBinop ((PrimUntyped.UBits2 (PrimUntyped.UCompare (false, CLt))),
+      (UVar ('t'::('r'::('g'::('_'::('x'::[])))))), (UVar
+      ('s'::('r'::('c'::('_'::('x'::[])))))))), (USugar (UCallModule
+      ((Obj.magic id), (Obj.magic __), (Obj.magic r0_send), ((UUnop
+      ((PrimUntyped.UConv PrimUntyped.UPack), (UBinop ((PrimUntyped.UStruct2
+      (PrimUntyped.USubstField ('s'::('r'::('c'::[]))))), (UVar
+      ('m'::('s'::('g'::[])))), (UVar
+      ('r'::('_'::('a'::('d'::('d'::('r'::[]))))))))))) :: [])))), (USugar
+      (UConstBits (0, (Obj.magic __)))))))))))))))))), (USugar (UConstBits
+      (0, (Obj.magic __)))))), (UBind (('m'::('s'::('g'::('1'::[])))), (UUnop
+      ((PrimUntyped.UConv (PrimUntyped.UUnpack (Struct_t Types.basic_flit))),
+      (UVar ('m'::('1'::[]))))), (UBind
+      (('n'::('e'::('w'::('_'::('d'::('a'::('t'::('a'::[])))))))), (UUnop
+      ((PrimUntyped.UStruct1 (PrimUntyped.UGetField
+      ('n'::('e'::('w'::[]))))), (UVar ('m'::('s'::('g'::('1'::[]))))))),
+      (UBind (('s'::('r'::('c'::('_'::('p'::[]))))), (UUnop
+      ((PrimUntyped.UStruct1 (PrimUntyped.UGetField
+      ('s'::('r'::('c'::[]))))), (UVar ('m'::('s'::('g'::('1'::[]))))))),
+      (UIf ((UBinop ((PrimUntyped.UBits2 PrimUntyped.UAnd), (UBinop
+      ((PrimUntyped.UEq true), (UVar ('s'::('r'::('c'::('_'::('p'::[])))))),
+      (UVar ('r'::('_'::('a'::('d'::('d'::('r'::[]))))))))), (UVar
+      ('n'::('e'::('w'::('_'::('d'::('a'::('t'::('a'::[]))))))))))), (USeq
+      ((USugar (UCallModule ((Obj.magic id), (Obj.magic __),
+      (Obj.magic r1_send), ((UUnop ((PrimUntyped.UConv PrimUntyped.UPack),
+      (UBinop ((PrimUntyped.UStruct2 (PrimUntyped.USubstField
+      ('n'::('e'::('w'::[]))))), (UVar ('m'::('s'::('g'::('1'::[]))))),
+      (USugar (UConstBits ((Stdlib.Int.succ 0),
       (vect_cons 0 false (Obj.magic __))))))))) :: [])))), (UBind
       (('t'::('r'::('g'::('_'::('x'::[]))))), (UUnop ((PrimUntyped.UStruct1
       (PrimUntyped.UGetField ('t'::('r'::('g'::('_'::('x'::[]))))))), (UVar
@@ -1934,49 +2119,66 @@ module Router =
       ('r'::('_'::('a'::('d'::('d'::('r'::[]))))))))))), (UIf ((UBinop
       ((PrimUntyped.UBits2 (PrimUntyped.UCompare (false, CGt))), (UVar
       ('t'::('r'::('g'::('_'::('x'::[])))))), (UVar
-      ('s'::('r'::('c'::('_'::('x'::[])))))))), (USugar (UCallModule ((Obj.magic id),
-      (Obj.magic __), (Obj.magic r1_send), ((UUnop ((PrimUntyped.UConv
-      PrimUntyped.UPack), (UBinop ((PrimUntyped.UStruct2 (PrimUntyped.USubstField
-      ('s'::('r'::('c'::[]))))), (UVar ('m'::('s'::('g'::('1'::[]))))), (UVar
-      ('r'::('_'::('a'::('d'::('d'::('r'::[]))))))))))) :: [])))), (UIf ((UBinop
-      ((PrimUntyped.UBits2 (PrimUntyped.UCompare (false, CLt))), (UVar
-      ('t'::('r'::('g'::('_'::('x'::[])))))), (UVar
-      ('s'::('r'::('c'::('_'::('x'::[])))))))), (USugar (UCallModule ((Obj.magic id),
-      (Obj.magic __), (Obj.magic r0_send), ((UUnop ((PrimUntyped.UConv
-      PrimUntyped.UPack), (UBinop ((PrimUntyped.UStruct2 (PrimUntyped.USubstField
-      ('s'::('r'::('c'::[]))))), (UVar ('m'::('s'::('g'::('1'::[]))))), (UVar
-      ('r'::('_'::('a'::('d'::('d'::('r'::[]))))))))))) :: [])))), (USugar (UConstBits
-      (0, (Obj.magic __)))))))))))))))))), (USugar (UConstBits (0,
-      (Obj.magic __)))))))))))))))))))))))))
+      ('s'::('r'::('c'::('_'::('x'::[])))))))), (USugar (UCallModule
+      ((Obj.magic id), (Obj.magic __), (Obj.magic r1_send), ((UUnop
+      ((PrimUntyped.UConv PrimUntyped.UPack), (UBinop ((PrimUntyped.UStruct2
+      (PrimUntyped.USubstField ('s'::('r'::('c'::[]))))), (UVar
+      ('m'::('s'::('g'::('1'::[]))))), (UVar
+      ('r'::('_'::('a'::('d'::('d'::('r'::[]))))))))))) :: [])))), (UIf
+      ((UBinop ((PrimUntyped.UBits2 (PrimUntyped.UCompare (false, CLt))),
+      (UVar ('t'::('r'::('g'::('_'::('x'::[])))))), (UVar
+      ('s'::('r'::('c'::('_'::('x'::[])))))))), (USugar (UCallModule
+      ((Obj.magic id), (Obj.magic __), (Obj.magic r0_send), ((UUnop
+      ((PrimUntyped.UConv PrimUntyped.UPack), (UBinop ((PrimUntyped.UStruct2
+      (PrimUntyped.USubstField ('s'::('r'::('c'::[]))))), (UVar
+      ('m'::('s'::('g'::('1'::[]))))), (UVar
+      ('r'::('_'::('a'::('d'::('d'::('r'::[]))))))))))) :: [])))), (USugar
+      (UConstBits (0, (Obj.magic __)))))))))))))))))), (USugar (UConstBits
+      (0, (Obj.magic __)))))))))))))))))))))))))
 
   (** val _routeend_r :
-      int -> (var_t, fn_name_t, (pos_t, var_t, fn_name_t, Regs.reg_t, __) uaction)
-      internalFunction -> (var_t, fn_name_t, (pos_t, var_t, fn_name_t, Regs.reg_t, __)
-      uaction) internalFunction -> (pos_t, var_t, fn_name_t, Regs.reg_t, __) uaction **)
+      int -> (var_t, fn_name_t, (pos_t, var_t, fn_name_t, Regs.reg_t, __)
+      uaction) internalFunction -> (var_t, fn_name_t, (pos_t, var_t,
+      fn_name_t, Regs.reg_t, __) uaction) internalFunction -> (pos_t, var_t,
+      fn_name_t, Regs.reg_t, __) uaction **)
 
   let _routeend_r r_addr2 r0_send r0_receive =
     UBind (('r'::('_'::('a'::('d'::('d'::('r'::[])))))), (USugar (UConstBits
-      ((Stdlib.Int.succ (Stdlib.Int.succ (Stdlib.Int.succ (Stdlib.Int.succ 0)))),
-      (Bits.of_nat (Stdlib.Int.succ (Stdlib.Int.succ (Stdlib.Int.succ (Stdlib.Int.succ
-        0)))) r_addr2)))), (UBind (('m'::('0'::[])), (USugar (UCallModule
-      ((Obj.magic id), (Obj.magic __), (Obj.magic r0_receive), []))), (UBind
-      (('m'::('s'::('g'::[]))), (UUnop ((PrimUntyped.UConv (PrimUntyped.UUnpack
-      (Struct_t Types.basic_flit))), (UVar ('m'::('0'::[]))))), (UBind
+      ((Stdlib.Int.succ (Stdlib.Int.succ (Stdlib.Int.succ (Stdlib.Int.succ
+      0)))),
+      (Bits.of_nat (Stdlib.Int.succ (Stdlib.Int.succ (Stdlib.Int.succ
+        (Stdlib.Int.succ 0)))) r_addr2)))), (UBind (('m'::('0'::[])), (UBinop
+      ((PrimUntyped.UBits2 PrimUntyped.UXor), (USugar (UCallModule
+      ((Obj.magic id), (Obj.magic __), (Obj.magic r0_receive), []))),
+      (UExternalCall (__, (USugar (UConstBits ((Stdlib.Int.succ
+      (Stdlib.Int.succ (Stdlib.Int.succ (Stdlib.Int.succ (Stdlib.Int.succ
+      (Stdlib.Int.succ (Stdlib.Int.succ (Stdlib.Int.succ (Stdlib.Int.succ
+      (Stdlib.Int.succ (Stdlib.Int.succ (Stdlib.Int.succ (Stdlib.Int.succ
+      (Stdlib.Int.succ 0)))))))))))))),
+      (Bits.of_N (Stdlib.Int.succ (Stdlib.Int.succ (Stdlib.Int.succ
+        (Stdlib.Int.succ (Stdlib.Int.succ (Stdlib.Int.succ (Stdlib.Int.succ
+        (Stdlib.Int.succ (Stdlib.Int.succ (Stdlib.Int.succ (Stdlib.Int.succ
+        (Stdlib.Int.succ (Stdlib.Int.succ (Stdlib.Int.succ 0)))))))))))))) 0)))))))),
+      (UBind (('m'::('s'::('g'::[]))), (UUnop ((PrimUntyped.UConv
+      (PrimUntyped.UUnpack (Struct_t Types.basic_flit))), (UVar
+      ('m'::('0'::[]))))), (UBind
       (('n'::('e'::('w'::('_'::('d'::('a'::('t'::('a'::[])))))))), (UUnop
-      ((PrimUntyped.UStruct1 (PrimUntyped.UGetField ('n'::('e'::('w'::[]))))), (UVar
-      ('m'::('s'::('g'::[])))))), (UBind (('s'::('r'::('c'::('_'::('p'::[]))))),
-      (UUnop ((PrimUntyped.UStruct1 (PrimUntyped.UGetField ('s'::('r'::('c'::[]))))),
-      (UVar ('m'::('s'::('g'::[])))))), (UIf ((UBinop ((PrimUntyped.UBits2
+      ((PrimUntyped.UStruct1 (PrimUntyped.UGetField
+      ('n'::('e'::('w'::[]))))), (UVar ('m'::('s'::('g'::[])))))), (UBind
+      (('s'::('r'::('c'::('_'::('p'::[]))))), (UUnop ((PrimUntyped.UStruct1
+      (PrimUntyped.UGetField ('s'::('r'::('c'::[]))))), (UVar
+      ('m'::('s'::('g'::[])))))), (UIf ((UBinop ((PrimUntyped.UBits2
       PrimUntyped.UAnd), (UBinop ((PrimUntyped.UEq true), (UVar
       ('s'::('r'::('c'::('_'::('p'::[])))))), (UVar
       ('r'::('_'::('a'::('d'::('d'::('r'::[]))))))))), (UVar
       ('n'::('e'::('w'::('_'::('d'::('a'::('t'::('a'::[]))))))))))), (UBind
       (('t'::('r'::('g'::('_'::('x'::[]))))), (UUnop ((PrimUntyped.UStruct1
       (PrimUntyped.UGetField ('t'::('r'::('g'::('_'::('x'::[]))))))), (UVar
-      ('m'::('s'::('g'::[])))))), (UBind (('t'::('r'::('g'::('_'::('y'::[]))))),
-      (UUnop ((PrimUntyped.UStruct1 (PrimUntyped.UGetField
-      ('t'::('r'::('g'::('_'::('y'::[]))))))), (UVar ('m'::('s'::('g'::[])))))),
-      (UBind (('s'::('r'::('c'::('_'::('x'::[]))))), (UUnop ((PrimUntyped.UStruct1
+      ('m'::('s'::('g'::[])))))), (UBind
+      (('t'::('r'::('g'::('_'::('y'::[]))))), (UUnop ((PrimUntyped.UStruct1
+      (PrimUntyped.UGetField ('t'::('r'::('g'::('_'::('y'::[]))))))), (UVar
+      ('m'::('s'::('g'::[])))))), (UBind
+      (('s'::('r'::('c'::('_'::('x'::[]))))), (UUnop ((PrimUntyped.UStruct1
       (PrimUntyped.UGetField ('x'::[]))), (UUnop ((PrimUntyped.UConv
       (PrimUntyped.UUnpack (Struct_t Types.router_address))), (UVar
       ('r'::('_'::('a'::('d'::('d'::('r'::[]))))))))))), (UBind
@@ -1986,20 +2188,21 @@ module Router =
       ('r'::('_'::('a'::('d'::('d'::('r'::[]))))))))))), (UIf ((UBinop
       ((PrimUntyped.UBits2 (PrimUntyped.UCompare (false, CGt))), (UVar
       ('t'::('r'::('g'::('_'::('x'::[])))))), (UVar
-      ('s'::('r'::('c'::('_'::('x'::[])))))))), (UFail (Bits_t 0)), (UIf ((UBinop
-      ((PrimUntyped.UBits2 (PrimUntyped.UCompare (false, CLt))), (UVar
-      ('t'::('r'::('g'::('_'::('x'::[])))))), (UVar
-      ('s'::('r'::('c'::('_'::('x'::[])))))))), (USugar (UCallModule ((Obj.magic id),
-      (Obj.magic __), (Obj.magic r0_send), ((UUnop ((PrimUntyped.UConv
-      PrimUntyped.UPack), (UBinop ((PrimUntyped.UStruct2 (PrimUntyped.USubstField
-      ('s'::('r'::('c'::[]))))), (UVar ('m'::('s'::('g'::[])))), (UVar
-      ('r'::('_'::('a'::('d'::('d'::('r'::[]))))))))))) :: [])))), (USugar (UConstBits
-      (0, (Obj.magic __)))))))))))))))), (USugar (UConstBits (0,
+      ('s'::('r'::('c'::('_'::('x'::[])))))))), (UFail (Bits_t 0)), (UIf
+      ((UBinop ((PrimUntyped.UBits2 (PrimUntyped.UCompare (false, CLt))),
+      (UVar ('t'::('r'::('g'::('_'::('x'::[])))))), (UVar
+      ('s'::('r'::('c'::('_'::('x'::[])))))))), (USugar (UCallModule
+      ((Obj.magic id), (Obj.magic __), (Obj.magic r0_send), ((UUnop
+      ((PrimUntyped.UConv PrimUntyped.UPack), (UBinop ((PrimUntyped.UStruct2
+      (PrimUntyped.USubstField ('s'::('r'::('c'::[]))))), (UVar
+      ('m'::('s'::('g'::[])))), (UVar
+      ('r'::('_'::('a'::('d'::('d'::('r'::[]))))))))))) :: [])))), (USugar
+      (UConstBits (0, (Obj.magic __)))))))))))))))), (USugar (UConstBits (0,
       (Obj.magic __)))))))))))))))
 
   (** val routecenterfn :
-      int -> Regs.reg_t -> Regs.reg_t -> (pos_t, var_t, fn_name_t, Regs.reg_t, __)
-      uaction **)
+      int -> Regs.reg_t -> Regs.reg_t -> (pos_t, var_t, fn_name_t,
+      Regs.reg_t, __) uaction **)
 
   let routecenterfn n0 r1 r2 =
     _routecenter_r n0 (r_send r1) (r_send r2) (r_receive r1) (r_receive r2)
@@ -2053,10 +2256,11 @@ module NOCImpl =
   (** val schedule : (pos_t, rule_name_t) scheduler **)
 
   let schedule =
-    Cons (Coq_router_4, (Cons (Coq_router_3, (Cons (Coq_router_2, (Cons (Coq_router_1,
-      Done)))))))
+    Cons (Coq_router_4, (Cons (Coq_router_3, (Cons (Coq_router_2, (Cons
+      (Coq_router_1, Done)))))))
 
-  (** val rules : rule_name_t -> (pos_t, var_t, fn_name_t, reg_t, __) action **)
+  (** val rules :
+      rule_name_t -> (pos_t, var_t, fn_name_t, reg_t, __) action **)
 
   let rules = function
   | Coq_router_1 ->
@@ -2064,358 +2268,495 @@ module NOCImpl =
       (let desugared =
          desugar_action dummyPos_unit.dummy_pos (UBind
            (('r'::('_'::('a'::('d'::('d'::('r'::[])))))), (USugar (UConstBits
-           ((Stdlib.Int.succ (Stdlib.Int.succ (Stdlib.Int.succ (Stdlib.Int.succ 0)))),
+           ((Stdlib.Int.succ (Stdlib.Int.succ (Stdlib.Int.succ
+           (Stdlib.Int.succ 0)))),
            (Bits.of_nat (Stdlib.Int.succ (Stdlib.Int.succ (Stdlib.Int.succ
-             (Stdlib.Int.succ 0)))) 0)))), (UBind (('m'::('0'::[])), (USugar
-           (UCallModule (id, (Obj.magic __), (Obj.magic Routerfns.r_receive Coq_r1),
-           []))), (UBind (('m'::('s'::('g'::[]))), (UUnop ((PrimUntyped.UConv
+             (Stdlib.Int.succ 0)))) 0)))), (UBind (('m'::('0'::[])), (UBinop
+           ((PrimUntyped.UBits2 PrimUntyped.UXor), (USugar (UCallModule (id,
+           (Obj.magic __), (Obj.magic Routerfns.r_receive Coq_r1), []))),
+           (UExternalCall (__, (USugar (UConstBits ((Stdlib.Int.succ
+           (Stdlib.Int.succ (Stdlib.Int.succ (Stdlib.Int.succ
+           (Stdlib.Int.succ (Stdlib.Int.succ (Stdlib.Int.succ
+           (Stdlib.Int.succ (Stdlib.Int.succ (Stdlib.Int.succ
+           (Stdlib.Int.succ (Stdlib.Int.succ (Stdlib.Int.succ
+           (Stdlib.Int.succ 0)))))))))))))),
+           (Bits.of_N (Stdlib.Int.succ (Stdlib.Int.succ (Stdlib.Int.succ
+             (Stdlib.Int.succ (Stdlib.Int.succ (Stdlib.Int.succ
+             (Stdlib.Int.succ (Stdlib.Int.succ (Stdlib.Int.succ
+             (Stdlib.Int.succ (Stdlib.Int.succ (Stdlib.Int.succ
+             (Stdlib.Int.succ (Stdlib.Int.succ 0)))))))))))))) 0)))))))),
+           (UBind (('m'::('s'::('g'::[]))), (UUnop ((PrimUntyped.UConv
            (PrimUntyped.UUnpack (Struct_t Types.basic_flit))), (UVar
            ('m'::('0'::[]))))), (UBind
-           (('n'::('e'::('w'::('_'::('d'::('a'::('t'::('a'::[])))))))), (UUnop
-           ((PrimUntyped.UStruct1 (PrimUntyped.UGetField ('n'::('e'::('w'::[]))))),
-           (UVar ('m'::('s'::('g'::[])))))), (UBind
-           (('s'::('r'::('c'::('_'::('p'::[]))))), (UUnop ((PrimUntyped.UStruct1
-           (PrimUntyped.UGetField ('s'::('r'::('c'::[]))))), (UVar
-           ('m'::('s'::('g'::[])))))), (UIf ((UBinop ((PrimUntyped.UBits2
-           PrimUntyped.UAnd), (UBinop ((PrimUntyped.UEq true), (UVar
+           (('n'::('e'::('w'::('_'::('d'::('a'::('t'::('a'::[])))))))),
+           (UUnop ((PrimUntyped.UStruct1 (PrimUntyped.UGetField
+           ('n'::('e'::('w'::[]))))), (UVar ('m'::('s'::('g'::[])))))),
+           (UBind (('s'::('r'::('c'::('_'::('p'::[]))))), (UUnop
+           ((PrimUntyped.UStruct1 (PrimUntyped.UGetField
+           ('s'::('r'::('c'::[]))))), (UVar ('m'::('s'::('g'::[])))))), (UIf
+           ((UBinop ((PrimUntyped.UBits2 PrimUntyped.UAnd), (UBinop
+           ((PrimUntyped.UEq true), (UVar
            ('s'::('r'::('c'::('_'::('p'::[])))))), (UVar
            ('r'::('_'::('a'::('d'::('d'::('r'::[]))))))))), (UVar
-           ('n'::('e'::('w'::('_'::('d'::('a'::('t'::('a'::[]))))))))))), (UBind
-           (('t'::('r'::('g'::('_'::('x'::[]))))), (UUnop ((PrimUntyped.UStruct1
-           (PrimUntyped.UGetField ('t'::('r'::('g'::('_'::('x'::[]))))))), (UVar
-           ('m'::('s'::('g'::[])))))), (UBind (('t'::('r'::('g'::('_'::('y'::[]))))),
-           (UUnop ((PrimUntyped.UStruct1 (PrimUntyped.UGetField
-           ('t'::('r'::('g'::('_'::('y'::[]))))))), (UVar ('m'::('s'::('g'::[])))))),
-           (UBind (('s'::('r'::('c'::('_'::('x'::[]))))), (UUnop
+           ('n'::('e'::('w'::('_'::('d'::('a'::('t'::('a'::[]))))))))))),
+           (UBind (('t'::('r'::('g'::('_'::('x'::[]))))), (UUnop
+           ((PrimUntyped.UStruct1 (PrimUntyped.UGetField
+           ('t'::('r'::('g'::('_'::('x'::[]))))))), (UVar
+           ('m'::('s'::('g'::[])))))), (UBind
+           (('t'::('r'::('g'::('_'::('y'::[]))))), (UUnop
+           ((PrimUntyped.UStruct1 (PrimUntyped.UGetField
+           ('t'::('r'::('g'::('_'::('y'::[]))))))), (UVar
+           ('m'::('s'::('g'::[])))))), (UBind
+           (('s'::('r'::('c'::('_'::('x'::[]))))), (UUnop
            ((PrimUntyped.UStruct1 (PrimUntyped.UGetField ('x'::[]))), (UUnop
-           ((PrimUntyped.UConv (PrimUntyped.UUnpack (Struct_t Types.router_address))),
-           (UVar ('r'::('_'::('a'::('d'::('d'::('r'::[]))))))))))), (UBind
-           (('s'::('r'::('c'::('_'::('y'::[]))))), (UUnop ((PrimUntyped.UStruct1
-           (PrimUntyped.UGetField ('y'::[]))), (UUnop ((PrimUntyped.UConv
-           (PrimUntyped.UUnpack (Struct_t Types.router_address))), (UVar
+           ((PrimUntyped.UConv (PrimUntyped.UUnpack (Struct_t
+           Types.router_address))), (UVar
+           ('r'::('_'::('a'::('d'::('d'::('r'::[]))))))))))), (UBind
+           (('s'::('r'::('c'::('_'::('y'::[]))))), (UUnop
+           ((PrimUntyped.UStruct1 (PrimUntyped.UGetField ('y'::[]))), (UUnop
+           ((PrimUntyped.UConv (PrimUntyped.UUnpack (Struct_t
+           Types.router_address))), (UVar
            ('r'::('_'::('a'::('d'::('d'::('r'::[]))))))))))), (UIf ((UBinop
            ((PrimUntyped.UBits2 (PrimUntyped.UCompare (false, CGt))), (UVar
            ('t'::('r'::('g'::('_'::('x'::[])))))), (UVar
-           ('s'::('r'::('c'::('_'::('x'::[])))))))), (USugar (UCallModule (id,
-           (Obj.magic __), (Obj.magic Routerfns.r_send Coq_r1), ((UUnop
-           ((PrimUntyped.UConv PrimUntyped.UPack), (UBinop ((PrimUntyped.UStruct2
-           (PrimUntyped.USubstField ('s'::('r'::('c'::[]))))), (UVar
-           ('m'::('s'::('g'::[])))), (UVar
-           ('r'::('_'::('a'::('d'::('d'::('r'::[]))))))))))) :: [])))), (UIf ((UBinop
-           ((PrimUntyped.UBits2 (PrimUntyped.UCompare (false, CLt))), (UVar
-           ('t'::('r'::('g'::('_'::('x'::[])))))), (UVar
-           ('s'::('r'::('c'::('_'::('x'::[])))))))), (UFail (Bits_t 0)), (USugar
-           (UConstBits (0, (Obj.magic __)))))))))))))))), (USugar (UConstBits (0,
-           (Obj.magic __))))))))))))))))
+           ('s'::('r'::('c'::('_'::('x'::[])))))))), (USugar (UCallModule
+           (id, (Obj.magic __), (Obj.magic Routerfns.r_send Coq_r1), ((UUnop
+           ((PrimUntyped.UConv PrimUntyped.UPack), (UBinop
+           ((PrimUntyped.UStruct2 (PrimUntyped.USubstField
+           ('s'::('r'::('c'::[]))))), (UVar ('m'::('s'::('g'::[])))), (UVar
+           ('r'::('_'::('a'::('d'::('d'::('r'::[]))))))))))) :: [])))), (UIf
+           ((UBinop ((PrimUntyped.UBits2 (PrimUntyped.UCompare (false,
+           CLt))), (UVar ('t'::('r'::('g'::('_'::('x'::[])))))), (UVar
+           ('s'::('r'::('c'::('_'::('x'::[])))))))), (UFail (Bits_t 0)),
+           (USugar (UConstBits (0, (Obj.magic __)))))))))))))))), (USugar
+           (UConstBits (0, (Obj.magic __))))))))))))))))
        in
-       tc_action eqDec_string coq_R empty_Sigma dummyPos_unit.dummy_pos [] (Bits_t 0)
-         (Obj.magic desugared))
+       tc_action eqDec_string coq_R Routerfns.coq_Sigma
+         dummyPos_unit.dummy_pos [] (Bits_t 0) (Obj.magic desugared))
   | Coq_router_2 ->
     extract_success
       (let desugared =
          desugar_action dummyPos_unit.dummy_pos (UBind
            (('r'::('_'::('a'::('d'::('d'::('r'::[])))))), (USugar (UConstBits
-           ((Stdlib.Int.succ (Stdlib.Int.succ (Stdlib.Int.succ (Stdlib.Int.succ 0)))),
+           ((Stdlib.Int.succ (Stdlib.Int.succ (Stdlib.Int.succ
+           (Stdlib.Int.succ 0)))),
            (Bits.of_nat (Stdlib.Int.succ (Stdlib.Int.succ (Stdlib.Int.succ
-             (Stdlib.Int.succ 0)))) (Stdlib.Int.succ 0))))), (UBind (('m'::('0'::[])),
+             (Stdlib.Int.succ 0)))) (Stdlib.Int.succ 0))))), (UBind
+           (('m'::('0'::[])), (UBinop ((PrimUntyped.UBits2 PrimUntyped.UXor),
            (USugar (UCallModule (id, (Obj.magic __),
-           (Obj.magic Routerfns.r_receive Coq_r1), []))), (UBind (('m'::('1'::[])),
-           (USugar (UCallModule (id, (Obj.magic __),
-           (Obj.magic Routerfns.r_receive Coq_r2), []))), (UBind
-           (('m'::('s'::('g'::[]))), (UUnop ((PrimUntyped.UConv (PrimUntyped.UUnpack
-           (Struct_t Types.basic_flit))), (UVar ('m'::('0'::[]))))), (UBind
-           (('n'::('e'::('w'::('_'::('d'::('a'::('t'::('a'::[])))))))), (UUnop
-           ((PrimUntyped.UStruct1 (PrimUntyped.UGetField ('n'::('e'::('w'::[]))))),
-           (UVar ('m'::('s'::('g'::[])))))), (UBind
-           (('s'::('r'::('c'::('_'::('p'::[]))))), (UUnop ((PrimUntyped.UStruct1
-           (PrimUntyped.UGetField ('s'::('r'::('c'::[]))))), (UVar
-           ('m'::('s'::('g'::[])))))), (USeq ((UIf ((UBinop ((PrimUntyped.UBits2
-           PrimUntyped.UAnd), (UBinop ((PrimUntyped.UEq true), (UVar
-           ('s'::('r'::('c'::('_'::('p'::[])))))), (UVar
-           ('r'::('_'::('a'::('d'::('d'::('r'::[]))))))))), (UVar
-           ('n'::('e'::('w'::('_'::('d'::('a'::('t'::('a'::[]))))))))))), (USeq
-           ((USugar (UCallModule (id, (Obj.magic __),
-           (Obj.magic Routerfns.r_send Coq_r1), ((UUnop ((PrimUntyped.UConv
-           PrimUntyped.UPack), (UBinop ((PrimUntyped.UStruct2 (PrimUntyped.USubstField
-           ('n'::('e'::('w'::[]))))), (UVar ('m'::('s'::('g'::[])))), (USugar
-           (UConstBits ((Stdlib.Int.succ 0),
-           (vect_cons 0 false (Obj.magic __))))))))) :: [])))), (UBind
-           (('t'::('r'::('g'::('_'::('x'::[]))))), (UUnop ((PrimUntyped.UStruct1
-           (PrimUntyped.UGetField ('t'::('r'::('g'::('_'::('x'::[]))))))), (UVar
-           ('m'::('s'::('g'::[])))))), (UBind (('t'::('r'::('g'::('_'::('y'::[]))))),
+           (Obj.magic Routerfns.r_receive Coq_r1), []))), (UExternalCall (__,
+           (USugar (UConstBits ((Stdlib.Int.succ (Stdlib.Int.succ
+           (Stdlib.Int.succ (Stdlib.Int.succ (Stdlib.Int.succ
+           (Stdlib.Int.succ (Stdlib.Int.succ (Stdlib.Int.succ
+           (Stdlib.Int.succ (Stdlib.Int.succ (Stdlib.Int.succ
+           (Stdlib.Int.succ (Stdlib.Int.succ (Stdlib.Int.succ
+           0)))))))))))))),
+           (Bits.of_N (Stdlib.Int.succ (Stdlib.Int.succ (Stdlib.Int.succ
+             (Stdlib.Int.succ (Stdlib.Int.succ (Stdlib.Int.succ
+             (Stdlib.Int.succ (Stdlib.Int.succ (Stdlib.Int.succ
+             (Stdlib.Int.succ (Stdlib.Int.succ (Stdlib.Int.succ
+             (Stdlib.Int.succ (Stdlib.Int.succ 0)))))))))))))) 0)))))))),
+           (UBind (('m'::('1'::[])), (UBinop ((PrimUntyped.UBits2
+           PrimUntyped.UXor), (USugar (UCallModule (id, (Obj.magic __),
+           (Obj.magic Routerfns.r_receive Coq_r2), []))), (UExternalCall (__,
+           (USugar (UConstBits ((Stdlib.Int.succ (Stdlib.Int.succ
+           (Stdlib.Int.succ (Stdlib.Int.succ (Stdlib.Int.succ
+           (Stdlib.Int.succ (Stdlib.Int.succ (Stdlib.Int.succ
+           (Stdlib.Int.succ (Stdlib.Int.succ (Stdlib.Int.succ
+           (Stdlib.Int.succ (Stdlib.Int.succ (Stdlib.Int.succ
+           0)))))))))))))),
+           (Bits.of_N (Stdlib.Int.succ (Stdlib.Int.succ (Stdlib.Int.succ
+             (Stdlib.Int.succ (Stdlib.Int.succ (Stdlib.Int.succ
+             (Stdlib.Int.succ (Stdlib.Int.succ (Stdlib.Int.succ
+             (Stdlib.Int.succ (Stdlib.Int.succ (Stdlib.Int.succ
+             (Stdlib.Int.succ (Stdlib.Int.succ 0)))))))))))))) 0)))))))),
+           (UBind (('m'::('s'::('g'::[]))), (UUnop ((PrimUntyped.UConv
+           (PrimUntyped.UUnpack (Struct_t Types.basic_flit))), (UVar
+           ('m'::('0'::[]))))), (UBind
+           (('n'::('e'::('w'::('_'::('d'::('a'::('t'::('a'::[])))))))),
            (UUnop ((PrimUntyped.UStruct1 (PrimUntyped.UGetField
-           ('t'::('r'::('g'::('_'::('y'::[]))))))), (UVar ('m'::('s'::('g'::[])))))),
-           (UBind (('s'::('r'::('c'::('_'::('x'::[]))))), (UUnop
-           ((PrimUntyped.UStruct1 (PrimUntyped.UGetField ('x'::[]))), (UUnop
-           ((PrimUntyped.UConv (PrimUntyped.UUnpack (Struct_t Types.router_address))),
-           (UVar ('r'::('_'::('a'::('d'::('d'::('r'::[]))))))))))), (UBind
-           (('s'::('r'::('c'::('_'::('y'::[]))))), (UUnop ((PrimUntyped.UStruct1
-           (PrimUntyped.UGetField ('y'::[]))), (UUnop ((PrimUntyped.UConv
-           (PrimUntyped.UUnpack (Struct_t Types.router_address))), (UVar
-           ('r'::('_'::('a'::('d'::('d'::('r'::[]))))))))))), (UIf ((UBinop
-           ((PrimUntyped.UBits2 (PrimUntyped.UCompare (false, CGt))), (UVar
-           ('t'::('r'::('g'::('_'::('x'::[])))))), (UVar
-           ('s'::('r'::('c'::('_'::('x'::[])))))))), (USugar (UCallModule (id,
-           (Obj.magic __), (Obj.magic Routerfns.r_send Coq_r2), ((UUnop
-           ((PrimUntyped.UConv PrimUntyped.UPack), (UBinop ((PrimUntyped.UStruct2
-           (PrimUntyped.USubstField ('s'::('r'::('c'::[]))))), (UVar
-           ('m'::('s'::('g'::[])))), (UVar
-           ('r'::('_'::('a'::('d'::('d'::('r'::[]))))))))))) :: [])))), (UIf ((UBinop
-           ((PrimUntyped.UBits2 (PrimUntyped.UCompare (false, CLt))), (UVar
-           ('t'::('r'::('g'::('_'::('x'::[])))))), (UVar
-           ('s'::('r'::('c'::('_'::('x'::[])))))))), (USugar (UCallModule (id,
-           (Obj.magic __), (Obj.magic Routerfns.r_send Coq_r1), ((UUnop
-           ((PrimUntyped.UConv PrimUntyped.UPack), (UBinop ((PrimUntyped.UStruct2
-           (PrimUntyped.USubstField ('s'::('r'::('c'::[]))))), (UVar
-           ('m'::('s'::('g'::[])))), (UVar
-           ('r'::('_'::('a'::('d'::('d'::('r'::[]))))))))))) :: [])))), (USugar
-           (UConstBits (0, (Obj.magic __)))))))))))))))))), (USugar (UConstBits (0,
-           (Obj.magic __)))))), (UBind (('m'::('s'::('g'::('1'::[])))), (UUnop
-           ((PrimUntyped.UConv (PrimUntyped.UUnpack (Struct_t Types.basic_flit))),
-           (UVar ('m'::('1'::[]))))), (UBind
-           (('n'::('e'::('w'::('_'::('d'::('a'::('t'::('a'::[])))))))), (UUnop
-           ((PrimUntyped.UStruct1 (PrimUntyped.UGetField ('n'::('e'::('w'::[]))))),
-           (UVar ('m'::('s'::('g'::('1'::[]))))))), (UBind
-           (('s'::('r'::('c'::('_'::('p'::[]))))), (UUnop ((PrimUntyped.UStruct1
-           (PrimUntyped.UGetField ('s'::('r'::('c'::[]))))), (UVar
-           ('m'::('s'::('g'::('1'::[]))))))), (UIf ((UBinop ((PrimUntyped.UBits2
-           PrimUntyped.UAnd), (UBinop ((PrimUntyped.UEq true), (UVar
+           ('n'::('e'::('w'::[]))))), (UVar ('m'::('s'::('g'::[])))))),
+           (UBind (('s'::('r'::('c'::('_'::('p'::[]))))), (UUnop
+           ((PrimUntyped.UStruct1 (PrimUntyped.UGetField
+           ('s'::('r'::('c'::[]))))), (UVar ('m'::('s'::('g'::[])))))), (USeq
+           ((UIf ((UBinop ((PrimUntyped.UBits2 PrimUntyped.UAnd), (UBinop
+           ((PrimUntyped.UEq true), (UVar
            ('s'::('r'::('c'::('_'::('p'::[])))))), (UVar
            ('r'::('_'::('a'::('d'::('d'::('r'::[]))))))))), (UVar
-           ('n'::('e'::('w'::('_'::('d'::('a'::('t'::('a'::[]))))))))))), (USeq
-           ((USugar (UCallModule (id, (Obj.magic __),
-           (Obj.magic Routerfns.r_send Coq_r2), ((UUnop ((PrimUntyped.UConv
-           PrimUntyped.UPack), (UBinop ((PrimUntyped.UStruct2 (PrimUntyped.USubstField
-           ('n'::('e'::('w'::[]))))), (UVar ('m'::('s'::('g'::('1'::[]))))), (USugar
-           (UConstBits ((Stdlib.Int.succ 0),
-           (vect_cons 0 false (Obj.magic __))))))))) :: [])))), (UBind
-           (('t'::('r'::('g'::('_'::('x'::[]))))), (UUnop ((PrimUntyped.UStruct1
-           (PrimUntyped.UGetField ('t'::('r'::('g'::('_'::('x'::[]))))))), (UVar
-           ('m'::('s'::('g'::('1'::[]))))))), (UBind
-           (('t'::('r'::('g'::('_'::('y'::[]))))), (UUnop ((PrimUntyped.UStruct1
-           (PrimUntyped.UGetField ('t'::('r'::('g'::('_'::('y'::[]))))))), (UVar
-           ('m'::('s'::('g'::('1'::[]))))))), (UBind
-           (('s'::('r'::('c'::('_'::('x'::[]))))), (UUnop ((PrimUntyped.UStruct1
-           (PrimUntyped.UGetField ('x'::[]))), (UUnop ((PrimUntyped.UConv
-           (PrimUntyped.UUnpack (Struct_t Types.router_address))), (UVar
+           ('n'::('e'::('w'::('_'::('d'::('a'::('t'::('a'::[]))))))))))),
+           (USeq ((USugar (UCallModule (id, (Obj.magic __),
+           (Obj.magic Routerfns.r_send Coq_r1), ((UUnop ((PrimUntyped.UConv
+           PrimUntyped.UPack), (UBinop ((PrimUntyped.UStruct2
+           (PrimUntyped.USubstField ('n'::('e'::('w'::[]))))), (UVar
+           ('m'::('s'::('g'::[])))), (USugar (UConstBits ((Stdlib.Int.succ
+           0), (vect_cons 0 false (Obj.magic __))))))))) :: [])))), (UBind
+           (('t'::('r'::('g'::('_'::('x'::[]))))), (UUnop
+           ((PrimUntyped.UStruct1 (PrimUntyped.UGetField
+           ('t'::('r'::('g'::('_'::('x'::[]))))))), (UVar
+           ('m'::('s'::('g'::[])))))), (UBind
+           (('t'::('r'::('g'::('_'::('y'::[]))))), (UUnop
+           ((PrimUntyped.UStruct1 (PrimUntyped.UGetField
+           ('t'::('r'::('g'::('_'::('y'::[]))))))), (UVar
+           ('m'::('s'::('g'::[])))))), (UBind
+           (('s'::('r'::('c'::('_'::('x'::[]))))), (UUnop
+           ((PrimUntyped.UStruct1 (PrimUntyped.UGetField ('x'::[]))), (UUnop
+           ((PrimUntyped.UConv (PrimUntyped.UUnpack (Struct_t
+           Types.router_address))), (UVar
            ('r'::('_'::('a'::('d'::('d'::('r'::[]))))))))))), (UBind
-           (('s'::('r'::('c'::('_'::('y'::[]))))), (UUnop ((PrimUntyped.UStruct1
-           (PrimUntyped.UGetField ('y'::[]))), (UUnop ((PrimUntyped.UConv
-           (PrimUntyped.UUnpack (Struct_t Types.router_address))), (UVar
+           (('s'::('r'::('c'::('_'::('y'::[]))))), (UUnop
+           ((PrimUntyped.UStruct1 (PrimUntyped.UGetField ('y'::[]))), (UUnop
+           ((PrimUntyped.UConv (PrimUntyped.UUnpack (Struct_t
+           Types.router_address))), (UVar
            ('r'::('_'::('a'::('d'::('d'::('r'::[]))))))))))), (UIf ((UBinop
            ((PrimUntyped.UBits2 (PrimUntyped.UCompare (false, CGt))), (UVar
            ('t'::('r'::('g'::('_'::('x'::[])))))), (UVar
-           ('s'::('r'::('c'::('_'::('x'::[])))))))), (USugar (UCallModule (id,
-           (Obj.magic __), (Obj.magic Routerfns.r_send Coq_r2), ((UUnop
-           ((PrimUntyped.UConv PrimUntyped.UPack), (UBinop ((PrimUntyped.UStruct2
-           (PrimUntyped.USubstField ('s'::('r'::('c'::[]))))), (UVar
-           ('m'::('s'::('g'::('1'::[]))))), (UVar
-           ('r'::('_'::('a'::('d'::('d'::('r'::[]))))))))))) :: [])))), (UIf ((UBinop
-           ((PrimUntyped.UBits2 (PrimUntyped.UCompare (false, CLt))), (UVar
+           ('s'::('r'::('c'::('_'::('x'::[])))))))), (USugar (UCallModule
+           (id, (Obj.magic __), (Obj.magic Routerfns.r_send Coq_r2), ((UUnop
+           ((PrimUntyped.UConv PrimUntyped.UPack), (UBinop
+           ((PrimUntyped.UStruct2 (PrimUntyped.USubstField
+           ('s'::('r'::('c'::[]))))), (UVar ('m'::('s'::('g'::[])))), (UVar
+           ('r'::('_'::('a'::('d'::('d'::('r'::[]))))))))))) :: [])))), (UIf
+           ((UBinop ((PrimUntyped.UBits2 (PrimUntyped.UCompare (false,
+           CLt))), (UVar ('t'::('r'::('g'::('_'::('x'::[])))))), (UVar
+           ('s'::('r'::('c'::('_'::('x'::[])))))))), (USugar (UCallModule
+           (id, (Obj.magic __), (Obj.magic Routerfns.r_send Coq_r1), ((UUnop
+           ((PrimUntyped.UConv PrimUntyped.UPack), (UBinop
+           ((PrimUntyped.UStruct2 (PrimUntyped.USubstField
+           ('s'::('r'::('c'::[]))))), (UVar ('m'::('s'::('g'::[])))), (UVar
+           ('r'::('_'::('a'::('d'::('d'::('r'::[]))))))))))) :: [])))),
+           (USugar (UConstBits (0, (Obj.magic __)))))))))))))))))), (USugar
+           (UConstBits (0, (Obj.magic __)))))), (UBind
+           (('m'::('s'::('g'::('1'::[])))), (UUnop ((PrimUntyped.UConv
+           (PrimUntyped.UUnpack (Struct_t Types.basic_flit))), (UVar
+           ('m'::('1'::[]))))), (UBind
+           (('n'::('e'::('w'::('_'::('d'::('a'::('t'::('a'::[])))))))),
+           (UUnop ((PrimUntyped.UStruct1 (PrimUntyped.UGetField
+           ('n'::('e'::('w'::[]))))), (UVar
+           ('m'::('s'::('g'::('1'::[]))))))), (UBind
+           (('s'::('r'::('c'::('_'::('p'::[]))))), (UUnop
+           ((PrimUntyped.UStruct1 (PrimUntyped.UGetField
+           ('s'::('r'::('c'::[]))))), (UVar
+           ('m'::('s'::('g'::('1'::[]))))))), (UIf ((UBinop
+           ((PrimUntyped.UBits2 PrimUntyped.UAnd), (UBinop ((PrimUntyped.UEq
+           true), (UVar ('s'::('r'::('c'::('_'::('p'::[])))))), (UVar
+           ('r'::('_'::('a'::('d'::('d'::('r'::[]))))))))), (UVar
+           ('n'::('e'::('w'::('_'::('d'::('a'::('t'::('a'::[]))))))))))),
+           (USeq ((USugar (UCallModule (id, (Obj.magic __),
+           (Obj.magic Routerfns.r_send Coq_r2), ((UUnop ((PrimUntyped.UConv
+           PrimUntyped.UPack), (UBinop ((PrimUntyped.UStruct2
+           (PrimUntyped.USubstField ('n'::('e'::('w'::[]))))), (UVar
+           ('m'::('s'::('g'::('1'::[]))))), (USugar (UConstBits
+           ((Stdlib.Int.succ 0),
+           (vect_cons 0 false (Obj.magic __))))))))) :: [])))), (UBind
+           (('t'::('r'::('g'::('_'::('x'::[]))))), (UUnop
+           ((PrimUntyped.UStruct1 (PrimUntyped.UGetField
+           ('t'::('r'::('g'::('_'::('x'::[]))))))), (UVar
+           ('m'::('s'::('g'::('1'::[]))))))), (UBind
+           (('t'::('r'::('g'::('_'::('y'::[]))))), (UUnop
+           ((PrimUntyped.UStruct1 (PrimUntyped.UGetField
+           ('t'::('r'::('g'::('_'::('y'::[]))))))), (UVar
+           ('m'::('s'::('g'::('1'::[]))))))), (UBind
+           (('s'::('r'::('c'::('_'::('x'::[]))))), (UUnop
+           ((PrimUntyped.UStruct1 (PrimUntyped.UGetField ('x'::[]))), (UUnop
+           ((PrimUntyped.UConv (PrimUntyped.UUnpack (Struct_t
+           Types.router_address))), (UVar
+           ('r'::('_'::('a'::('d'::('d'::('r'::[]))))))))))), (UBind
+           (('s'::('r'::('c'::('_'::('y'::[]))))), (UUnop
+           ((PrimUntyped.UStruct1 (PrimUntyped.UGetField ('y'::[]))), (UUnop
+           ((PrimUntyped.UConv (PrimUntyped.UUnpack (Struct_t
+           Types.router_address))), (UVar
+           ('r'::('_'::('a'::('d'::('d'::('r'::[]))))))))))), (UIf ((UBinop
+           ((PrimUntyped.UBits2 (PrimUntyped.UCompare (false, CGt))), (UVar
            ('t'::('r'::('g'::('_'::('x'::[])))))), (UVar
-           ('s'::('r'::('c'::('_'::('x'::[])))))))), (USugar (UCallModule (id,
-           (Obj.magic __), (Obj.magic Routerfns.r_send Coq_r1), ((UUnop
-           ((PrimUntyped.UConv PrimUntyped.UPack), (UBinop ((PrimUntyped.UStruct2
-           (PrimUntyped.USubstField ('s'::('r'::('c'::[]))))), (UVar
-           ('m'::('s'::('g'::('1'::[]))))), (UVar
-           ('r'::('_'::('a'::('d'::('d'::('r'::[]))))))))))) :: [])))), (USugar
-           (UConstBits (0, (Obj.magic __)))))))))))))))))), (USugar (UConstBits (0,
-           (Obj.magic __))))))))))))))))))))))))))
+           ('s'::('r'::('c'::('_'::('x'::[])))))))), (USugar (UCallModule
+           (id, (Obj.magic __), (Obj.magic Routerfns.r_send Coq_r2), ((UUnop
+           ((PrimUntyped.UConv PrimUntyped.UPack), (UBinop
+           ((PrimUntyped.UStruct2 (PrimUntyped.USubstField
+           ('s'::('r'::('c'::[]))))), (UVar ('m'::('s'::('g'::('1'::[]))))),
+           (UVar ('r'::('_'::('a'::('d'::('d'::('r'::[]))))))))))) :: [])))),
+           (UIf ((UBinop ((PrimUntyped.UBits2 (PrimUntyped.UCompare (false,
+           CLt))), (UVar ('t'::('r'::('g'::('_'::('x'::[])))))), (UVar
+           ('s'::('r'::('c'::('_'::('x'::[])))))))), (USugar (UCallModule
+           (id, (Obj.magic __), (Obj.magic Routerfns.r_send Coq_r1), ((UUnop
+           ((PrimUntyped.UConv PrimUntyped.UPack), (UBinop
+           ((PrimUntyped.UStruct2 (PrimUntyped.USubstField
+           ('s'::('r'::('c'::[]))))), (UVar ('m'::('s'::('g'::('1'::[]))))),
+           (UVar ('r'::('_'::('a'::('d'::('d'::('r'::[]))))))))))) :: [])))),
+           (USugar (UConstBits (0, (Obj.magic __)))))))))))))))))), (USugar
+           (UConstBits (0, (Obj.magic __))))))))))))))))))))))))))
        in
-       tc_action eqDec_string coq_R empty_Sigma dummyPos_unit.dummy_pos [] (Bits_t 0)
-         (Obj.magic desugared))
+       tc_action eqDec_string coq_R Routerfns.coq_Sigma
+         dummyPos_unit.dummy_pos [] (Bits_t 0) (Obj.magic desugared))
   | Coq_router_3 ->
     extract_success
       (let desugared =
          desugar_action dummyPos_unit.dummy_pos (UBind
            (('r'::('_'::('a'::('d'::('d'::('r'::[])))))), (USugar (UConstBits
-           ((Stdlib.Int.succ (Stdlib.Int.succ (Stdlib.Int.succ (Stdlib.Int.succ 0)))),
+           ((Stdlib.Int.succ (Stdlib.Int.succ (Stdlib.Int.succ
+           (Stdlib.Int.succ 0)))),
            (Bits.of_nat (Stdlib.Int.succ (Stdlib.Int.succ (Stdlib.Int.succ
-             (Stdlib.Int.succ 0)))) (Stdlib.Int.succ (Stdlib.Int.succ 0)))))), (UBind
-           (('m'::('0'::[])), (USugar (UCallModule (id, (Obj.magic __),
-           (Obj.magic Routerfns.r_receive Coq_r2), []))), (UBind (('m'::('1'::[])),
-           (USugar (UCallModule (id, (Obj.magic __),
-           (Obj.magic Routerfns.r_receive Coq_r3), []))), (UBind
-           (('m'::('s'::('g'::[]))), (UUnop ((PrimUntyped.UConv (PrimUntyped.UUnpack
-           (Struct_t Types.basic_flit))), (UVar ('m'::('0'::[]))))), (UBind
-           (('n'::('e'::('w'::('_'::('d'::('a'::('t'::('a'::[])))))))), (UUnop
-           ((PrimUntyped.UStruct1 (PrimUntyped.UGetField ('n'::('e'::('w'::[]))))),
-           (UVar ('m'::('s'::('g'::[])))))), (UBind
-           (('s'::('r'::('c'::('_'::('p'::[]))))), (UUnop ((PrimUntyped.UStruct1
-           (PrimUntyped.UGetField ('s'::('r'::('c'::[]))))), (UVar
-           ('m'::('s'::('g'::[])))))), (USeq ((UIf ((UBinop ((PrimUntyped.UBits2
-           PrimUntyped.UAnd), (UBinop ((PrimUntyped.UEq true), (UVar
-           ('s'::('r'::('c'::('_'::('p'::[])))))), (UVar
-           ('r'::('_'::('a'::('d'::('d'::('r'::[]))))))))), (UVar
-           ('n'::('e'::('w'::('_'::('d'::('a'::('t'::('a'::[]))))))))))), (USeq
-           ((USugar (UCallModule (id, (Obj.magic __),
-           (Obj.magic Routerfns.r_send Coq_r2), ((UUnop ((PrimUntyped.UConv
-           PrimUntyped.UPack), (UBinop ((PrimUntyped.UStruct2 (PrimUntyped.USubstField
-           ('n'::('e'::('w'::[]))))), (UVar ('m'::('s'::('g'::[])))), (USugar
-           (UConstBits ((Stdlib.Int.succ 0),
-           (vect_cons 0 false (Obj.magic __))))))))) :: [])))), (UBind
-           (('t'::('r'::('g'::('_'::('x'::[]))))), (UUnop ((PrimUntyped.UStruct1
-           (PrimUntyped.UGetField ('t'::('r'::('g'::('_'::('x'::[]))))))), (UVar
-           ('m'::('s'::('g'::[])))))), (UBind (('t'::('r'::('g'::('_'::('y'::[]))))),
+             (Stdlib.Int.succ 0)))) (Stdlib.Int.succ (Stdlib.Int.succ 0)))))),
+           (UBind (('m'::('0'::[])), (UBinop ((PrimUntyped.UBits2
+           PrimUntyped.UXor), (USugar (UCallModule (id, (Obj.magic __),
+           (Obj.magic Routerfns.r_receive Coq_r2), []))), (UExternalCall (__,
+           (USugar (UConstBits ((Stdlib.Int.succ (Stdlib.Int.succ
+           (Stdlib.Int.succ (Stdlib.Int.succ (Stdlib.Int.succ
+           (Stdlib.Int.succ (Stdlib.Int.succ (Stdlib.Int.succ
+           (Stdlib.Int.succ (Stdlib.Int.succ (Stdlib.Int.succ
+           (Stdlib.Int.succ (Stdlib.Int.succ (Stdlib.Int.succ
+           0)))))))))))))),
+           (Bits.of_N (Stdlib.Int.succ (Stdlib.Int.succ (Stdlib.Int.succ
+             (Stdlib.Int.succ (Stdlib.Int.succ (Stdlib.Int.succ
+             (Stdlib.Int.succ (Stdlib.Int.succ (Stdlib.Int.succ
+             (Stdlib.Int.succ (Stdlib.Int.succ (Stdlib.Int.succ
+             (Stdlib.Int.succ (Stdlib.Int.succ 0)))))))))))))) 0)))))))),
+           (UBind (('m'::('1'::[])), (UBinop ((PrimUntyped.UBits2
+           PrimUntyped.UXor), (USugar (UCallModule (id, (Obj.magic __),
+           (Obj.magic Routerfns.r_receive Coq_r3), []))), (UExternalCall (__,
+           (USugar (UConstBits ((Stdlib.Int.succ (Stdlib.Int.succ
+           (Stdlib.Int.succ (Stdlib.Int.succ (Stdlib.Int.succ
+           (Stdlib.Int.succ (Stdlib.Int.succ (Stdlib.Int.succ
+           (Stdlib.Int.succ (Stdlib.Int.succ (Stdlib.Int.succ
+           (Stdlib.Int.succ (Stdlib.Int.succ (Stdlib.Int.succ
+           0)))))))))))))),
+           (Bits.of_N (Stdlib.Int.succ (Stdlib.Int.succ (Stdlib.Int.succ
+             (Stdlib.Int.succ (Stdlib.Int.succ (Stdlib.Int.succ
+             (Stdlib.Int.succ (Stdlib.Int.succ (Stdlib.Int.succ
+             (Stdlib.Int.succ (Stdlib.Int.succ (Stdlib.Int.succ
+             (Stdlib.Int.succ (Stdlib.Int.succ 0)))))))))))))) 0)))))))),
+           (UBind (('m'::('s'::('g'::[]))), (UUnop ((PrimUntyped.UConv
+           (PrimUntyped.UUnpack (Struct_t Types.basic_flit))), (UVar
+           ('m'::('0'::[]))))), (UBind
+           (('n'::('e'::('w'::('_'::('d'::('a'::('t'::('a'::[])))))))),
            (UUnop ((PrimUntyped.UStruct1 (PrimUntyped.UGetField
-           ('t'::('r'::('g'::('_'::('y'::[]))))))), (UVar ('m'::('s'::('g'::[])))))),
-           (UBind (('s'::('r'::('c'::('_'::('x'::[]))))), (UUnop
-           ((PrimUntyped.UStruct1 (PrimUntyped.UGetField ('x'::[]))), (UUnop
-           ((PrimUntyped.UConv (PrimUntyped.UUnpack (Struct_t Types.router_address))),
-           (UVar ('r'::('_'::('a'::('d'::('d'::('r'::[]))))))))))), (UBind
-           (('s'::('r'::('c'::('_'::('y'::[]))))), (UUnop ((PrimUntyped.UStruct1
-           (PrimUntyped.UGetField ('y'::[]))), (UUnop ((PrimUntyped.UConv
-           (PrimUntyped.UUnpack (Struct_t Types.router_address))), (UVar
-           ('r'::('_'::('a'::('d'::('d'::('r'::[]))))))))))), (UIf ((UBinop
-           ((PrimUntyped.UBits2 (PrimUntyped.UCompare (false, CGt))), (UVar
-           ('t'::('r'::('g'::('_'::('x'::[])))))), (UVar
-           ('s'::('r'::('c'::('_'::('x'::[])))))))), (USugar (UCallModule (id,
-           (Obj.magic __), (Obj.magic Routerfns.r_send Coq_r3), ((UUnop
-           ((PrimUntyped.UConv PrimUntyped.UPack), (UBinop ((PrimUntyped.UStruct2
-           (PrimUntyped.USubstField ('s'::('r'::('c'::[]))))), (UVar
-           ('m'::('s'::('g'::[])))), (UVar
-           ('r'::('_'::('a'::('d'::('d'::('r'::[]))))))))))) :: [])))), (UIf ((UBinop
-           ((PrimUntyped.UBits2 (PrimUntyped.UCompare (false, CLt))), (UVar
-           ('t'::('r'::('g'::('_'::('x'::[])))))), (UVar
-           ('s'::('r'::('c'::('_'::('x'::[])))))))), (USugar (UCallModule (id,
-           (Obj.magic __), (Obj.magic Routerfns.r_send Coq_r2), ((UUnop
-           ((PrimUntyped.UConv PrimUntyped.UPack), (UBinop ((PrimUntyped.UStruct2
-           (PrimUntyped.USubstField ('s'::('r'::('c'::[]))))), (UVar
-           ('m'::('s'::('g'::[])))), (UVar
-           ('r'::('_'::('a'::('d'::('d'::('r'::[]))))))))))) :: [])))), (USugar
-           (UConstBits (0, (Obj.magic __)))))))))))))))))), (USugar (UConstBits (0,
-           (Obj.magic __)))))), (UBind (('m'::('s'::('g'::('1'::[])))), (UUnop
-           ((PrimUntyped.UConv (PrimUntyped.UUnpack (Struct_t Types.basic_flit))),
-           (UVar ('m'::('1'::[]))))), (UBind
-           (('n'::('e'::('w'::('_'::('d'::('a'::('t'::('a'::[])))))))), (UUnop
-           ((PrimUntyped.UStruct1 (PrimUntyped.UGetField ('n'::('e'::('w'::[]))))),
-           (UVar ('m'::('s'::('g'::('1'::[]))))))), (UBind
-           (('s'::('r'::('c'::('_'::('p'::[]))))), (UUnop ((PrimUntyped.UStruct1
-           (PrimUntyped.UGetField ('s'::('r'::('c'::[]))))), (UVar
-           ('m'::('s'::('g'::('1'::[]))))))), (UIf ((UBinop ((PrimUntyped.UBits2
-           PrimUntyped.UAnd), (UBinop ((PrimUntyped.UEq true), (UVar
+           ('n'::('e'::('w'::[]))))), (UVar ('m'::('s'::('g'::[])))))),
+           (UBind (('s'::('r'::('c'::('_'::('p'::[]))))), (UUnop
+           ((PrimUntyped.UStruct1 (PrimUntyped.UGetField
+           ('s'::('r'::('c'::[]))))), (UVar ('m'::('s'::('g'::[])))))), (USeq
+           ((UIf ((UBinop ((PrimUntyped.UBits2 PrimUntyped.UAnd), (UBinop
+           ((PrimUntyped.UEq true), (UVar
            ('s'::('r'::('c'::('_'::('p'::[])))))), (UVar
            ('r'::('_'::('a'::('d'::('d'::('r'::[]))))))))), (UVar
-           ('n'::('e'::('w'::('_'::('d'::('a'::('t'::('a'::[]))))))))))), (USeq
-           ((USugar (UCallModule (id, (Obj.magic __),
-           (Obj.magic Routerfns.r_send Coq_r3), ((UUnop ((PrimUntyped.UConv
-           PrimUntyped.UPack), (UBinop ((PrimUntyped.UStruct2 (PrimUntyped.USubstField
-           ('n'::('e'::('w'::[]))))), (UVar ('m'::('s'::('g'::('1'::[]))))), (USugar
-           (UConstBits ((Stdlib.Int.succ 0),
-           (vect_cons 0 false (Obj.magic __))))))))) :: [])))), (UBind
-           (('t'::('r'::('g'::('_'::('x'::[]))))), (UUnop ((PrimUntyped.UStruct1
-           (PrimUntyped.UGetField ('t'::('r'::('g'::('_'::('x'::[]))))))), (UVar
-           ('m'::('s'::('g'::('1'::[]))))))), (UBind
-           (('t'::('r'::('g'::('_'::('y'::[]))))), (UUnop ((PrimUntyped.UStruct1
-           (PrimUntyped.UGetField ('t'::('r'::('g'::('_'::('y'::[]))))))), (UVar
-           ('m'::('s'::('g'::('1'::[]))))))), (UBind
-           (('s'::('r'::('c'::('_'::('x'::[]))))), (UUnop ((PrimUntyped.UStruct1
-           (PrimUntyped.UGetField ('x'::[]))), (UUnop ((PrimUntyped.UConv
-           (PrimUntyped.UUnpack (Struct_t Types.router_address))), (UVar
+           ('n'::('e'::('w'::('_'::('d'::('a'::('t'::('a'::[]))))))))))),
+           (USeq ((USugar (UCallModule (id, (Obj.magic __),
+           (Obj.magic Routerfns.r_send Coq_r2), ((UUnop ((PrimUntyped.UConv
+           PrimUntyped.UPack), (UBinop ((PrimUntyped.UStruct2
+           (PrimUntyped.USubstField ('n'::('e'::('w'::[]))))), (UVar
+           ('m'::('s'::('g'::[])))), (USugar (UConstBits ((Stdlib.Int.succ
+           0), (vect_cons 0 false (Obj.magic __))))))))) :: [])))), (UBind
+           (('t'::('r'::('g'::('_'::('x'::[]))))), (UUnop
+           ((PrimUntyped.UStruct1 (PrimUntyped.UGetField
+           ('t'::('r'::('g'::('_'::('x'::[]))))))), (UVar
+           ('m'::('s'::('g'::[])))))), (UBind
+           (('t'::('r'::('g'::('_'::('y'::[]))))), (UUnop
+           ((PrimUntyped.UStruct1 (PrimUntyped.UGetField
+           ('t'::('r'::('g'::('_'::('y'::[]))))))), (UVar
+           ('m'::('s'::('g'::[])))))), (UBind
+           (('s'::('r'::('c'::('_'::('x'::[]))))), (UUnop
+           ((PrimUntyped.UStruct1 (PrimUntyped.UGetField ('x'::[]))), (UUnop
+           ((PrimUntyped.UConv (PrimUntyped.UUnpack (Struct_t
+           Types.router_address))), (UVar
            ('r'::('_'::('a'::('d'::('d'::('r'::[]))))))))))), (UBind
-           (('s'::('r'::('c'::('_'::('y'::[]))))), (UUnop ((PrimUntyped.UStruct1
-           (PrimUntyped.UGetField ('y'::[]))), (UUnop ((PrimUntyped.UConv
-           (PrimUntyped.UUnpack (Struct_t Types.router_address))), (UVar
+           (('s'::('r'::('c'::('_'::('y'::[]))))), (UUnop
+           ((PrimUntyped.UStruct1 (PrimUntyped.UGetField ('y'::[]))), (UUnop
+           ((PrimUntyped.UConv (PrimUntyped.UUnpack (Struct_t
+           Types.router_address))), (UVar
            ('r'::('_'::('a'::('d'::('d'::('r'::[]))))))))))), (UIf ((UBinop
            ((PrimUntyped.UBits2 (PrimUntyped.UCompare (false, CGt))), (UVar
            ('t'::('r'::('g'::('_'::('x'::[])))))), (UVar
-           ('s'::('r'::('c'::('_'::('x'::[])))))))), (USugar (UCallModule (id,
-           (Obj.magic __), (Obj.magic Routerfns.r_send Coq_r3), ((UUnop
-           ((PrimUntyped.UConv PrimUntyped.UPack), (UBinop ((PrimUntyped.UStruct2
-           (PrimUntyped.USubstField ('s'::('r'::('c'::[]))))), (UVar
-           ('m'::('s'::('g'::('1'::[]))))), (UVar
-           ('r'::('_'::('a'::('d'::('d'::('r'::[]))))))))))) :: [])))), (UIf ((UBinop
-           ((PrimUntyped.UBits2 (PrimUntyped.UCompare (false, CLt))), (UVar
+           ('s'::('r'::('c'::('_'::('x'::[])))))))), (USugar (UCallModule
+           (id, (Obj.magic __), (Obj.magic Routerfns.r_send Coq_r3), ((UUnop
+           ((PrimUntyped.UConv PrimUntyped.UPack), (UBinop
+           ((PrimUntyped.UStruct2 (PrimUntyped.USubstField
+           ('s'::('r'::('c'::[]))))), (UVar ('m'::('s'::('g'::[])))), (UVar
+           ('r'::('_'::('a'::('d'::('d'::('r'::[]))))))))))) :: [])))), (UIf
+           ((UBinop ((PrimUntyped.UBits2 (PrimUntyped.UCompare (false,
+           CLt))), (UVar ('t'::('r'::('g'::('_'::('x'::[])))))), (UVar
+           ('s'::('r'::('c'::('_'::('x'::[])))))))), (USugar (UCallModule
+           (id, (Obj.magic __), (Obj.magic Routerfns.r_send Coq_r2), ((UUnop
+           ((PrimUntyped.UConv PrimUntyped.UPack), (UBinop
+           ((PrimUntyped.UStruct2 (PrimUntyped.USubstField
+           ('s'::('r'::('c'::[]))))), (UVar ('m'::('s'::('g'::[])))), (UVar
+           ('r'::('_'::('a'::('d'::('d'::('r'::[]))))))))))) :: [])))),
+           (USugar (UConstBits (0, (Obj.magic __)))))))))))))))))), (USugar
+           (UConstBits (0, (Obj.magic __)))))), (UBind
+           (('m'::('s'::('g'::('1'::[])))), (UUnop ((PrimUntyped.UConv
+           (PrimUntyped.UUnpack (Struct_t Types.basic_flit))), (UVar
+           ('m'::('1'::[]))))), (UBind
+           (('n'::('e'::('w'::('_'::('d'::('a'::('t'::('a'::[])))))))),
+           (UUnop ((PrimUntyped.UStruct1 (PrimUntyped.UGetField
+           ('n'::('e'::('w'::[]))))), (UVar
+           ('m'::('s'::('g'::('1'::[]))))))), (UBind
+           (('s'::('r'::('c'::('_'::('p'::[]))))), (UUnop
+           ((PrimUntyped.UStruct1 (PrimUntyped.UGetField
+           ('s'::('r'::('c'::[]))))), (UVar
+           ('m'::('s'::('g'::('1'::[]))))))), (UIf ((UBinop
+           ((PrimUntyped.UBits2 PrimUntyped.UAnd), (UBinop ((PrimUntyped.UEq
+           true), (UVar ('s'::('r'::('c'::('_'::('p'::[])))))), (UVar
+           ('r'::('_'::('a'::('d'::('d'::('r'::[]))))))))), (UVar
+           ('n'::('e'::('w'::('_'::('d'::('a'::('t'::('a'::[]))))))))))),
+           (USeq ((USugar (UCallModule (id, (Obj.magic __),
+           (Obj.magic Routerfns.r_send Coq_r3), ((UUnop ((PrimUntyped.UConv
+           PrimUntyped.UPack), (UBinop ((PrimUntyped.UStruct2
+           (PrimUntyped.USubstField ('n'::('e'::('w'::[]))))), (UVar
+           ('m'::('s'::('g'::('1'::[]))))), (USugar (UConstBits
+           ((Stdlib.Int.succ 0),
+           (vect_cons 0 false (Obj.magic __))))))))) :: [])))), (UBind
+           (('t'::('r'::('g'::('_'::('x'::[]))))), (UUnop
+           ((PrimUntyped.UStruct1 (PrimUntyped.UGetField
+           ('t'::('r'::('g'::('_'::('x'::[]))))))), (UVar
+           ('m'::('s'::('g'::('1'::[]))))))), (UBind
+           (('t'::('r'::('g'::('_'::('y'::[]))))), (UUnop
+           ((PrimUntyped.UStruct1 (PrimUntyped.UGetField
+           ('t'::('r'::('g'::('_'::('y'::[]))))))), (UVar
+           ('m'::('s'::('g'::('1'::[]))))))), (UBind
+           (('s'::('r'::('c'::('_'::('x'::[]))))), (UUnop
+           ((PrimUntyped.UStruct1 (PrimUntyped.UGetField ('x'::[]))), (UUnop
+           ((PrimUntyped.UConv (PrimUntyped.UUnpack (Struct_t
+           Types.router_address))), (UVar
+           ('r'::('_'::('a'::('d'::('d'::('r'::[]))))))))))), (UBind
+           (('s'::('r'::('c'::('_'::('y'::[]))))), (UUnop
+           ((PrimUntyped.UStruct1 (PrimUntyped.UGetField ('y'::[]))), (UUnop
+           ((PrimUntyped.UConv (PrimUntyped.UUnpack (Struct_t
+           Types.router_address))), (UVar
+           ('r'::('_'::('a'::('d'::('d'::('r'::[]))))))))))), (UIf ((UBinop
+           ((PrimUntyped.UBits2 (PrimUntyped.UCompare (false, CGt))), (UVar
            ('t'::('r'::('g'::('_'::('x'::[])))))), (UVar
-           ('s'::('r'::('c'::('_'::('x'::[])))))))), (USugar (UCallModule (id,
-           (Obj.magic __), (Obj.magic Routerfns.r_send Coq_r2), ((UUnop
-           ((PrimUntyped.UConv PrimUntyped.UPack), (UBinop ((PrimUntyped.UStruct2
-           (PrimUntyped.USubstField ('s'::('r'::('c'::[]))))), (UVar
-           ('m'::('s'::('g'::('1'::[]))))), (UVar
-           ('r'::('_'::('a'::('d'::('d'::('r'::[]))))))))))) :: [])))), (USugar
-           (UConstBits (0, (Obj.magic __)))))))))))))))))), (USugar (UConstBits (0,
-           (Obj.magic __))))))))))))))))))))))))))
+           ('s'::('r'::('c'::('_'::('x'::[])))))))), (USugar (UCallModule
+           (id, (Obj.magic __), (Obj.magic Routerfns.r_send Coq_r3), ((UUnop
+           ((PrimUntyped.UConv PrimUntyped.UPack), (UBinop
+           ((PrimUntyped.UStruct2 (PrimUntyped.USubstField
+           ('s'::('r'::('c'::[]))))), (UVar ('m'::('s'::('g'::('1'::[]))))),
+           (UVar ('r'::('_'::('a'::('d'::('d'::('r'::[]))))))))))) :: [])))),
+           (UIf ((UBinop ((PrimUntyped.UBits2 (PrimUntyped.UCompare (false,
+           CLt))), (UVar ('t'::('r'::('g'::('_'::('x'::[])))))), (UVar
+           ('s'::('r'::('c'::('_'::('x'::[])))))))), (USugar (UCallModule
+           (id, (Obj.magic __), (Obj.magic Routerfns.r_send Coq_r2), ((UUnop
+           ((PrimUntyped.UConv PrimUntyped.UPack), (UBinop
+           ((PrimUntyped.UStruct2 (PrimUntyped.USubstField
+           ('s'::('r'::('c'::[]))))), (UVar ('m'::('s'::('g'::('1'::[]))))),
+           (UVar ('r'::('_'::('a'::('d'::('d'::('r'::[]))))))))))) :: [])))),
+           (USugar (UConstBits (0, (Obj.magic __)))))))))))))))))), (USugar
+           (UConstBits (0, (Obj.magic __))))))))))))))))))))))))))
        in
-       tc_action eqDec_string coq_R empty_Sigma dummyPos_unit.dummy_pos [] (Bits_t 0)
-         (Obj.magic desugared))
+       tc_action eqDec_string coq_R Routerfns.coq_Sigma
+         dummyPos_unit.dummy_pos [] (Bits_t 0) (Obj.magic desugared))
   | Coq_router_4 ->
     extract_success
       (let desugared =
          desugar_action dummyPos_unit.dummy_pos (UBind
            (('r'::('_'::('a'::('d'::('d'::('r'::[])))))), (USugar (UConstBits
-           ((Stdlib.Int.succ (Stdlib.Int.succ (Stdlib.Int.succ (Stdlib.Int.succ 0)))),
+           ((Stdlib.Int.succ (Stdlib.Int.succ (Stdlib.Int.succ
+           (Stdlib.Int.succ 0)))),
            (Bits.of_nat (Stdlib.Int.succ (Stdlib.Int.succ (Stdlib.Int.succ
-             (Stdlib.Int.succ 0)))) (Stdlib.Int.succ (Stdlib.Int.succ (Stdlib.Int.succ
-             0))))))), (UBind (('m'::('0'::[])), (USugar (UCallModule (id,
-           (Obj.magic __), (Obj.magic Routerfns.r_receive Coq_r3), []))), (UBind
-           (('m'::('s'::('g'::[]))), (UUnop ((PrimUntyped.UConv (PrimUntyped.UUnpack
-           (Struct_t Types.basic_flit))), (UVar ('m'::('0'::[]))))), (UBind
-           (('n'::('e'::('w'::('_'::('d'::('a'::('t'::('a'::[])))))))), (UUnop
-           ((PrimUntyped.UStruct1 (PrimUntyped.UGetField ('n'::('e'::('w'::[]))))),
-           (UVar ('m'::('s'::('g'::[])))))), (UBind
-           (('s'::('r'::('c'::('_'::('p'::[]))))), (UUnop ((PrimUntyped.UStruct1
-           (PrimUntyped.UGetField ('s'::('r'::('c'::[]))))), (UVar
-           ('m'::('s'::('g'::[])))))), (UIf ((UBinop ((PrimUntyped.UBits2
-           PrimUntyped.UAnd), (UBinop ((PrimUntyped.UEq true), (UVar
+             (Stdlib.Int.succ 0)))) (Stdlib.Int.succ (Stdlib.Int.succ
+             (Stdlib.Int.succ 0))))))), (UBind (('m'::('0'::[])), (UBinop
+           ((PrimUntyped.UBits2 PrimUntyped.UXor), (USugar (UCallModule (id,
+           (Obj.magic __), (Obj.magic Routerfns.r_receive Coq_r3), []))),
+           (UExternalCall (__, (USugar (UConstBits ((Stdlib.Int.succ
+           (Stdlib.Int.succ (Stdlib.Int.succ (Stdlib.Int.succ
+           (Stdlib.Int.succ (Stdlib.Int.succ (Stdlib.Int.succ
+           (Stdlib.Int.succ (Stdlib.Int.succ (Stdlib.Int.succ
+           (Stdlib.Int.succ (Stdlib.Int.succ (Stdlib.Int.succ
+           (Stdlib.Int.succ 0)))))))))))))),
+           (Bits.of_N (Stdlib.Int.succ (Stdlib.Int.succ (Stdlib.Int.succ
+             (Stdlib.Int.succ (Stdlib.Int.succ (Stdlib.Int.succ
+             (Stdlib.Int.succ (Stdlib.Int.succ (Stdlib.Int.succ
+             (Stdlib.Int.succ (Stdlib.Int.succ (Stdlib.Int.succ
+             (Stdlib.Int.succ (Stdlib.Int.succ 0)))))))))))))) 0)))))))),
+           (UBind (('m'::('s'::('g'::[]))), (UUnop ((PrimUntyped.UConv
+           (PrimUntyped.UUnpack (Struct_t Types.basic_flit))), (UVar
+           ('m'::('0'::[]))))), (UBind
+           (('n'::('e'::('w'::('_'::('d'::('a'::('t'::('a'::[])))))))),
+           (UUnop ((PrimUntyped.UStruct1 (PrimUntyped.UGetField
+           ('n'::('e'::('w'::[]))))), (UVar ('m'::('s'::('g'::[])))))),
+           (UBind (('s'::('r'::('c'::('_'::('p'::[]))))), (UUnop
+           ((PrimUntyped.UStruct1 (PrimUntyped.UGetField
+           ('s'::('r'::('c'::[]))))), (UVar ('m'::('s'::('g'::[])))))), (UIf
+           ((UBinop ((PrimUntyped.UBits2 PrimUntyped.UAnd), (UBinop
+           ((PrimUntyped.UEq true), (UVar
            ('s'::('r'::('c'::('_'::('p'::[])))))), (UVar
            ('r'::('_'::('a'::('d'::('d'::('r'::[]))))))))), (UVar
-           ('n'::('e'::('w'::('_'::('d'::('a'::('t'::('a'::[]))))))))))), (UBind
-           (('t'::('r'::('g'::('_'::('x'::[]))))), (UUnop ((PrimUntyped.UStruct1
-           (PrimUntyped.UGetField ('t'::('r'::('g'::('_'::('x'::[]))))))), (UVar
-           ('m'::('s'::('g'::[])))))), (UBind (('t'::('r'::('g'::('_'::('y'::[]))))),
-           (UUnop ((PrimUntyped.UStruct1 (PrimUntyped.UGetField
-           ('t'::('r'::('g'::('_'::('y'::[]))))))), (UVar ('m'::('s'::('g'::[])))))),
-           (UBind (('s'::('r'::('c'::('_'::('x'::[]))))), (UUnop
+           ('n'::('e'::('w'::('_'::('d'::('a'::('t'::('a'::[]))))))))))),
+           (UBind (('t'::('r'::('g'::('_'::('x'::[]))))), (UUnop
+           ((PrimUntyped.UStruct1 (PrimUntyped.UGetField
+           ('t'::('r'::('g'::('_'::('x'::[]))))))), (UVar
+           ('m'::('s'::('g'::[])))))), (UBind
+           (('t'::('r'::('g'::('_'::('y'::[]))))), (UUnop
+           ((PrimUntyped.UStruct1 (PrimUntyped.UGetField
+           ('t'::('r'::('g'::('_'::('y'::[]))))))), (UVar
+           ('m'::('s'::('g'::[])))))), (UBind
+           (('s'::('r'::('c'::('_'::('x'::[]))))), (UUnop
            ((PrimUntyped.UStruct1 (PrimUntyped.UGetField ('x'::[]))), (UUnop
-           ((PrimUntyped.UConv (PrimUntyped.UUnpack (Struct_t Types.router_address))),
-           (UVar ('r'::('_'::('a'::('d'::('d'::('r'::[]))))))))))), (UBind
-           (('s'::('r'::('c'::('_'::('y'::[]))))), (UUnop ((PrimUntyped.UStruct1
-           (PrimUntyped.UGetField ('y'::[]))), (UUnop ((PrimUntyped.UConv
-           (PrimUntyped.UUnpack (Struct_t Types.router_address))), (UVar
+           ((PrimUntyped.UConv (PrimUntyped.UUnpack (Struct_t
+           Types.router_address))), (UVar
+           ('r'::('_'::('a'::('d'::('d'::('r'::[]))))))))))), (UBind
+           (('s'::('r'::('c'::('_'::('y'::[]))))), (UUnop
+           ((PrimUntyped.UStruct1 (PrimUntyped.UGetField ('y'::[]))), (UUnop
+           ((PrimUntyped.UConv (PrimUntyped.UUnpack (Struct_t
+           Types.router_address))), (UVar
            ('r'::('_'::('a'::('d'::('d'::('r'::[]))))))))))), (UIf ((UBinop
            ((PrimUntyped.UBits2 (PrimUntyped.UCompare (false, CGt))), (UVar
            ('t'::('r'::('g'::('_'::('x'::[])))))), (UVar
-           ('s'::('r'::('c'::('_'::('x'::[])))))))), (UFail (Bits_t 0)), (UIf ((UBinop
-           ((PrimUntyped.UBits2 (PrimUntyped.UCompare (false, CLt))), (UVar
-           ('t'::('r'::('g'::('_'::('x'::[])))))), (UVar
-           ('s'::('r'::('c'::('_'::('x'::[])))))))), (USugar (UCallModule (id,
-           (Obj.magic __), (Obj.magic Routerfns.r_send Coq_r3), ((UUnop
-           ((PrimUntyped.UConv PrimUntyped.UPack), (UBinop ((PrimUntyped.UStruct2
-           (PrimUntyped.USubstField ('s'::('r'::('c'::[]))))), (UVar
-           ('m'::('s'::('g'::[])))), (UVar
-           ('r'::('_'::('a'::('d'::('d'::('r'::[]))))))))))) :: [])))), (USugar
-           (UConstBits (0, (Obj.magic __)))))))))))))))), (USugar (UConstBits (0,
-           (Obj.magic __))))))))))))))))
+           ('s'::('r'::('c'::('_'::('x'::[])))))))), (UFail (Bits_t 0)), (UIf
+           ((UBinop ((PrimUntyped.UBits2 (PrimUntyped.UCompare (false,
+           CLt))), (UVar ('t'::('r'::('g'::('_'::('x'::[])))))), (UVar
+           ('s'::('r'::('c'::('_'::('x'::[])))))))), (USugar (UCallModule
+           (id, (Obj.magic __), (Obj.magic Routerfns.r_send Coq_r3), ((UUnop
+           ((PrimUntyped.UConv PrimUntyped.UPack), (UBinop
+           ((PrimUntyped.UStruct2 (PrimUntyped.USubstField
+           ('s'::('r'::('c'::[]))))), (UVar ('m'::('s'::('g'::[])))), (UVar
+           ('r'::('_'::('a'::('d'::('d'::('r'::[]))))))))))) :: [])))),
+           (USugar (UConstBits (0, (Obj.magic __)))))))))))))))), (USugar
+           (UConstBits (0, (Obj.magic __))))))))))))))))
        in
-       tc_action eqDec_string coq_R empty_Sigma dummyPos_unit.dummy_pos [] (Bits_t 0)
-         (Obj.magic desugared))
+       tc_action eqDec_string coq_R Routerfns.coq_Sigma
+         dummyPos_unit.dummy_pos [] (Bits_t 0) (Obj.magic desugared))
+
+  (** val cpp_extfuns : char list **)
+
+  let cpp_extfuns =
+    'c'::('l'::('a'::('s'::('s'::(' '::('e'::('x'::('t'::('f'::('u'::('n'::('s'::(' '::('{'::('\n'::('p'::('u'::('b'::('l'::('i'::('c'::(':'::('\n'::(' '::(' '::('s'::('t'::('a'::('t'::('i'::('c'::(' '::('b'::('i'::('t'::('s'::('<'::('3'::('2'::('>'::(' '::('t'::('i'::('l'::('e'::('_'::('i'::('n'::('t'::('f'::('('::('b'::('i'::('t'::('s'::('<'::('3'::('2'::('>'::(' '::('s'::('t'::(')'::(' '::('{'::('\n'::(' '::(' '::(' '::(' '::('r'::('e'::('t'::('u'::('r'::('n'::(' '::('s'::('t'::(';'::('\n'::(' '::(' '::('}'::('\n'::('}'::(';'::[])))))))))))))))))))))))))))))))))))))))))))))))))))))))))))))))))))))))))))))))))))))))
+
+  (** val ext_fn_names : __ -> char list **)
+
+  let ext_fn_names _ =
+    't'::('i'::('l'::('e'::('_'::('i'::('n'::('t'::('f'::[]))))))))
 
   (** val package : interop_package_t **)
 
   let package =
-    { ip_koika = { koika_var_names = show_string; koika_fn_names = show_string;
-      koika_reg_names = { show0 = (fun h ->
+    { ip_koika = { koika_var_names = show_string; koika_fn_names =
+      show_string; koika_reg_names = { show0 = (fun h ->
       match Obj.magic h with
       | Coq_r1 -> 'r'::('1'::[])
       | Coq_r2 -> 'r'::('2'::[])
       | Coq_r3 -> 'r'::('3'::[])) }; koika_reg_types = (Obj.magic coq_R);
-      koika_reg_init = (Obj.magic r); koika_reg_finite = { finite_index = (fun h ->
+      koika_reg_init = (Obj.magic r); koika_reg_finite = { finite_index =
+      (fun h ->
       match Obj.magic h with
       | Coq_r1 -> 0
       | Coq_r2 -> Stdlib.Int.succ 0
       | Coq_r3 -> Stdlib.Int.succ (Stdlib.Int.succ 0)); finite_elements =
       ((Obj.magic Coq_r1) :: ((Obj.magic Coq_r2) :: ((Obj.magic Coq_r3) :: []))) };
-      koika_ext_fn_types = (Obj.magic empty_Sigma); koika_rules = (Obj.magic rules);
-      koika_rule_external = (fun _ -> false); koika_rule_names = { show0 = (fun h ->
+      koika_ext_fn_types = (Obj.magic Routerfns.coq_Sigma); koika_rules =
+      (Obj.magic rules); koika_rule_external = (fun _ -> false);
+      koika_rule_names = { show0 = (fun h ->
       match Obj.magic h with
-      | Coq_router_1 -> 'r'::('o'::('u'::('t'::('e'::('r'::('_'::('1'::[])))))))
-      | Coq_router_2 -> 'r'::('o'::('u'::('t'::('e'::('r'::('_'::('2'::[])))))))
-      | Coq_router_3 -> 'r'::('o'::('u'::('t'::('e'::('r'::('_'::('3'::[])))))))
-      | Coq_router_4 -> 'r'::('o'::('u'::('t'::('e'::('r'::('_'::('4'::[])))))))) };
+      | Coq_router_1 ->
+        'r'::('o'::('u'::('t'::('e'::('r'::('_'::('1'::[])))))))
+      | Coq_router_2 ->
+        'r'::('o'::('u'::('t'::('e'::('r'::('_'::('2'::[])))))))
+      | Coq_router_3 ->
+        'r'::('o'::('u'::('t'::('e'::('r'::('_'::('3'::[])))))))
+      | Coq_router_4 ->
+        'r'::('o'::('u'::('t'::('e'::('r'::('_'::('4'::[])))))))) };
       koika_scheduler = (Obj.magic schedule); koika_module_name =
       ('N'::('o'::('C'::[]))) }; ip_verilog = { vp_ext_fn_specs =
-      (Obj.magic empty_ext_fn_props) }; ip_sim = { sp_ext_fn_specs =
-      (Obj.magic empty_ext_fn_props); sp_prelude = None } }
+      (Obj.magic (fun _ -> { efr_name = (ext_fn_names __); efr_internal =
+        false })) }; ip_sim = { sp_ext_fn_specs =
+      (Obj.magic (fun _ -> { efs_name = (ext_fn_names __); efs_method =
+        false })); sp_prelude = (Some cpp_extfuns) } }
 
   (** val prog : unit **)
 
