noc_compiled/NoC.cpp
@@ -1,7 +1,12 @@
 /*! Default driver for Kôika programs compiled to C++ using Cuttlesim !*/
 #include "NoC.hpp"
 
-struct extfuns {};
+class extfuns {
+public:
+  static bits<32> tile_intf(bits<32> st) {
+    return st;
+  }
+};
 class simulator final : public module_NoC<extfuns> {};
 
 #ifdef SIM_MINIMAL
