noc_compiled/NoC.hpp
@@ -280,28 +280,32 @@ return true;
 DEF_RULE(router_3) {
 bits<4> r_addr = 4'0010_b;
 bits<14> m0 = CALL_FN(r_receive_0);
+bits<14> _y0 = extfuns.tile_intf(14'0_b);
+m0 = (m0 ^ _y0);
 bits<14> m1 = CALL_FN(r_receive_1);
+bits<14> _y1 = extfuns.tile_intf(14'0_b);
+m1 = (m1 ^ _y1);
 struct_basic_flit msg = prims::unpack<struct_basic_flit>(m0);
 bits<1> new_data = msg.renamed_cppnew;
 bits<4> src_p = msg.src;
 if (((src_p != r_addr) & new_data)) {
-struct_basic_flit _x4 = msg;
-_x4.renamed_cppnew = 1'0_b;
-CALL_FN(r_send_0, prims::pack(_x4));
+struct_basic_flit _x6 = msg;
+_x6.renamed_cppnew = 1'0_b;
+CALL_FN(r_send_0, prims::pack(_x6));
 bits<2> trg_x = msg.trg_x;
 bits<2> trg_y = msg.trg_y;
 bits<2> src_x = prims::unpack<struct_router_address>(r_addr).x;
 bits<2> src_y = prims::unpack<struct_router_address>(r_addr).y;
 if ((trg_x > src_x)) {
-struct_basic_flit _x12 = msg;
-_x12.src = r_addr;
-CALL_FN(r_send_1, prims::pack(_x12));
+struct_basic_flit _x14 = msg;
+_x14.src = r_addr;
+CALL_FN(r_send_1, prims::pack(_x14));
 }
 else {
 if ((trg_x < src_x)) {
-struct_basic_flit _x14 = msg;
-_x14.src = r_addr;
-CALL_FN(r_send_2, prims::pack(_x14));
+struct_basic_flit _x16 = msg;
+_x16.src = r_addr;
+CALL_FN(r_send_2, prims::pack(_x16));
 }
 }
 }
@@ -310,23 +314,23 @@ struct_basic_flit msg1 = prims::unpack<struct_basic_flit>(m1);
 bits<1> new_data = msg1.renamed_cppnew;
 bits<4> src_p = msg1.src;
 if (((src_p != r_addr) & new_data)) {
-struct_basic_flit _x19 = msg1;
-_x19.renamed_cppnew = 1'0_b;
-CALL_FN(r_send_3, prims::pack(_x19));
+struct_basic_flit _x21 = msg1;
+_x21.renamed_cppnew = 1'0_b;
+CALL_FN(r_send_3, prims::pack(_x21));
 bits<2> trg_x = msg1.trg_x;
 bits<2> trg_y = msg1.trg_y;
 bits<2> src_x = prims::unpack<struct_router_address>(r_addr).x;
 bits<2> src_y = prims::unpack<struct_router_address>(r_addr).y;
 if ((trg_x > src_x)) {
-struct_basic_flit _x27 = msg1;
-_x27.src = r_addr;
-CALL_FN(r_send_4, prims::pack(_x27));
+struct_basic_flit _x29 = msg1;
+_x29.src = r_addr;
+CALL_FN(r_send_4, prims::pack(_x29));
 }
 else {
 if ((trg_x < src_x)) {
-struct_basic_flit _x29 = msg1;
-_x29.src = r_addr;
-CALL_FN(r_send_5, prims::pack(_x29));
+struct_basic_flit _x31 = msg1;
+_x31.src = r_addr;
+CALL_FN(r_send_5, prims::pack(_x31));
 }
 }
 }
@@ -362,6 +366,8 @@ return true;
 DEF_RULE(router_4) {
 bits<4> r_addr = 4'0011_b;
 bits<14> m0 = CALL_FN(r_receive_2);
+bits<14> _y0 = extfuns.tile_intf(14'0_b);
+m0 = (m0 ^ _y0);
 struct_basic_flit msg = prims::unpack<struct_basic_flit>(m0);
 bits<1> new_data = msg.renamed_cppnew;
 bits<4> src_p = msg.src;
@@ -375,9 +381,9 @@ FAIL_FAST();
 }
 else {
 if ((trg_x < src_x)) {
-struct_basic_flit _x12 = msg;
-_x12.src = r_addr;
-CALL_FN(r_send_6, prims::pack(_x12));
+struct_basic_flit _x13 = msg;
+_x13.src = r_addr;
+CALL_FN(r_send_6, prims::pack(_x13));
 }
 }
 }
@@ -412,6 +418,8 @@ return true;
 DEF_RULE(router_1) {
 bits<4> r_addr = 4'0000_b;
 bits<14> m0 = CALL_FN(r_receive_3);
+bits<14> _y0 = extfuns.tile_intf(14'0_b);
+m0 = (m0 ^ _y0);
 struct_basic_flit msg = prims::unpack<struct_basic_flit>(m0);
 bits<1> new_data = msg.renamed_cppnew;
 bits<4> src_p = msg.src;
@@ -421,9 +429,9 @@ bits<2> trg_y = msg.trg_y;
 bits<2> src_x = prims::unpack<struct_router_address>(r_addr).x;
 bits<2> src_y = prims::unpack<struct_router_address>(r_addr).y;
 if ((trg_x > src_x)) {
-struct_basic_flit _x11 = msg;
-_x11.src = r_addr;
-CALL_FN(r_send_7, prims::pack(_x11));
+struct_basic_flit _x12 = msg;
+_x12.src = r_addr;
+CALL_FN(r_send_7, prims::pack(_x12));
 }
 else {
 if ((trg_x < src_x)) {
@@ -507,28 +515,32 @@ return true;
 DEF_RULE(router_2) {
 bits<4> r_addr = 4'0001_b;
 bits<14> m0 = CALL_FN(r_receive_4);
+bits<14> _y0 = extfuns.tile_intf(14'0_b);
+m0 = (m0 ^ _y0);
 bits<14> m1 = CALL_FN(r_receive_5);
+bits<14> _y1 = extfuns.tile_intf(14'0_b);
+m1 = (m1 ^ _y1);
 struct_basic_flit msg = prims::unpack<struct_basic_flit>(m0);
 bits<1> new_data = msg.renamed_cppnew;
 bits<4> src_p = msg.src;
 if (((src_p != r_addr) & new_data)) {
-struct_basic_flit _x4 = msg;
-_x4.renamed_cppnew = 1'0_b;
-CALL_FN(r_send_8, prims::pack(_x4));
+struct_basic_flit _x6 = msg;
+_x6.renamed_cppnew = 1'0_b;
+CALL_FN(r_send_8, prims::pack(_x6));
 bits<2> trg_x = msg.trg_x;
 bits<2> trg_y = msg.trg_y;
 bits<2> src_x = prims::unpack<struct_router_address>(r_addr).x;
 bits<2> src_y = prims::unpack<struct_router_address>(r_addr).y;
 if ((trg_x > src_x)) {
-struct_basic_flit _x12 = msg;
-_x12.src = r_addr;
-CALL_FN(r_send_9, prims::pack(_x12));
+struct_basic_flit _x14 = msg;
+_x14.src = r_addr;
+CALL_FN(r_send_9, prims::pack(_x14));
 }
 else {
 if ((trg_x < src_x)) {
-struct_basic_flit _x14 = msg;
-_x14.src = r_addr;
-CALL_FN(r_send_10, prims::pack(_x14));
+struct_basic_flit _x16 = msg;
+_x16.src = r_addr;
+CALL_FN(r_send_10, prims::pack(_x16));
 }
 }
 }
@@ -537,23 +549,23 @@ struct_basic_flit msg1 = prims::unpack<struct_basic_flit>(m1);
 bits<1> new_data = msg1.renamed_cppnew;
 bits<4> src_p = msg1.src;
 if (((src_p != r_addr) & new_data)) {
-struct_basic_flit _x19 = msg1;
-_x19.renamed_cppnew = 1'0_b;
-CALL_FN(r_send_11, prims::pack(_x19));
+struct_basic_flit _x21 = msg1;
+_x21.renamed_cppnew = 1'0_b;
+CALL_FN(r_send_11, prims::pack(_x21));
 bits<2> trg_x = msg1.trg_x;
 bits<2> trg_y = msg1.trg_y;
 bits<2> src_x = prims::unpack<struct_router_address>(r_addr).x;
 bits<2> src_y = prims::unpack<struct_router_address>(r_addr).y;
 if ((trg_x > src_x)) {
-struct_basic_flit _x27 = msg1;
-_x27.src = r_addr;
-CALL_FN(r_send_12, prims::pack(_x27));
+struct_basic_flit _x29 = msg1;
+_x29.src = r_addr;
+CALL_FN(r_send_12, prims::pack(_x29));
 }
 else {
 if ((trg_x < src_x)) {
-struct_basic_flit _x29 = msg1;
-_x29.src = r_addr;
-CALL_FN(r_send_13, prims::pack(_x29));
+struct_basic_flit _x31 = msg1;
+_x31.src = r_addr;
+CALL_FN(r_send_13, prims::pack(_x31));
 }
 }
 }
